thesis/BisimulationUptoScript.sml
@@ -38,15 +38,14 @@ val STRONG_BISIM_UPTO = new_definition (
 
 val IDENTITY_STRONG_BISIM_UPTO_lemma = store_thm (
    "IDENTITY_STRONG_BISIM_UPTO_lemma",
-  ``!E. (STRONG_EQUIV O (\x y. x = y) O STRONG_EQUIV) E E``,
-    GEN_TAC >> REWRITE_TAC [O_DEF] >> BETA_TAC
+  ``!E. (STRONG_EQUIV O Id O STRONG_EQUIV) E E``,
+    GEN_TAC >> REWRITE_TAC [O_DEF]
  >> NTAC 2 (Q.EXISTS_TAC `E` >> REWRITE_TAC [STRONG_EQUIV_REFL]));
 
 val IDENTITY_STRONG_BISIM_UPTO = store_thm (
-   "IDENTITY_STRONG_BISIM_UPTO", ``STRONG_BISIM_UPTO (\x y. x = y)``,
+   "IDENTITY_STRONG_BISIM_UPTO", ``STRONG_BISIM_UPTO Id``,
     PURE_ONCE_REWRITE_TAC [STRONG_BISIM_UPTO]
- >> BETA_TAC
- >> REPEAT STRIP_TAC (* 2 sub-goals *)
+ >> rpt STRIP_TAC (* 2 sub-goals *)
  >| [ (* goal 1 *)
       ASSUME_TAC (REWRITE_RULE [ASSUME ``E:('a, 'b) CCS = E'``]
 			       (ASSUME ``TRANS E u E1``)) \\
@@ -60,39 +59,37 @@ val IDENTITY_STRONG_BISIM_UPTO = store_thm (
       REWRITE_TAC [IDENTITY_STRONG_BISIM_UPTO_lemma] ]);
 
 val CONVERSE_STRONG_BISIM_UPTO_lemma = Q.prove (
-   `!Wbsm E E'. (STRONG_EQUIV O (\x y. Wbsm y x) O STRONG_EQUIV) E E' =
+   `!Wbsm E E'. (STRONG_EQUIV O (inv Wbsm) O STRONG_EQUIV) E E' =
 		(STRONG_EQUIV O Wbsm O STRONG_EQUIV) E' E`,
     rpt GEN_TAC
  >> EQ_TAC (* 2 sub-goals here *)
  >| [ (* goal 1 (of 2) *)
-      REWRITE_TAC [O_DEF] >> BETA_TAC >> rpt STRIP_TAC \\
+      REWRITE_TAC [O_DEF, inv_DEF] >> BETA_TAC >> rpt STRIP_TAC \\
       `STRONG_EQUIV y' E` by PROVE_TAC [STRONG_EQUIV_SYM] \\
       `STRONG_EQUIV E' y` by PROVE_TAC [STRONG_EQUIV_SYM] \\
-      Q.EXISTS_TAC `y'` >> ASM_REWRITE_TAC [] \\
-      Q.EXISTS_TAC `y` >> ASM_REWRITE_TAC [],
+      Q.EXISTS_TAC `y'` >> art [] \\
+      Q.EXISTS_TAC `y` >> art [],
       (* goal 2 (of 2) *)
-      REWRITE_TAC [O_DEF] >> BETA_TAC >> rpt STRIP_TAC \\
+      REWRITE_TAC [O_DEF, inv_DEF] >> BETA_TAC >> rpt STRIP_TAC \\
       `STRONG_EQUIV E y` by PROVE_TAC [STRONG_EQUIV_SYM] \\
       `STRONG_EQUIV y' E'` by PROVE_TAC [STRONG_EQUIV_SYM] \\
-      Q.EXISTS_TAC `y'` >> ASM_REWRITE_TAC [] \\
-      Q.EXISTS_TAC `y` >> ASM_REWRITE_TAC [] ]);
+      Q.EXISTS_TAC `y'` >> art [] \\
+      Q.EXISTS_TAC `y` >> art [] ]);
 
 val CONVERSE_STRONG_BISIM_UPTO = store_thm (
    "CONVERSE_STRONG_BISIM_UPTO",
-  ``!Wbsm. STRONG_BISIM_UPTO Wbsm ==> STRONG_BISIM_UPTO (\x y. Wbsm y x)``,
+  ``!Wbsm. STRONG_BISIM_UPTO Wbsm ==> STRONG_BISIM_UPTO (inv Wbsm)``,
     GEN_TAC
  >> PURE_ONCE_REWRITE_TAC [STRONG_BISIM_UPTO]
- >> BETA_TAC
+ >> REWRITE_TAC [inv_DEF] >> BETA_TAC
  >> rpt STRIP_TAC
  >> RES_TAC (* 2 sub-goals here *)
  >| [ (* goal 1 (of 2) *)
-      Q.EXISTS_TAC `E1'` >> ASM_REWRITE_TAC [] \\
-      REWRITE_TAC [CONVERSE_STRONG_BISIM_UPTO_lemma] \\
-      ASM_REWRITE_TAC [],
+      Q.EXISTS_TAC `E1'` >> art [] \\
+      REWRITE_TAC [CONVERSE_STRONG_BISIM_UPTO_lemma] >> art [],
       (* goal 2 (of 2) *)
-      Q.EXISTS_TAC `E2'` >> ASM_REWRITE_TAC [] \\
-      REWRITE_TAC [CONVERSE_STRONG_BISIM_UPTO_lemma] \\
-      ASM_REWRITE_TAC [] ]);
+      Q.EXISTS_TAC `E2'` >> art [] \\
+      REWRITE_TAC [CONVERSE_STRONG_BISIM_UPTO_lemma] >> art [] ]);
 
 val STRONG_BISIM_UPTO_LEMMA = store_thm (
    "STRONG_BISIM_UPTO_LEMMA",
@@ -126,9 +123,9 @@ val STRONG_BISIM_UPTO_LEMMA = store_thm (
  ***)
       `STRONG_EQUIV E1 y'''` by PROVE_TAC [STRONG_EQUIV_TRANS] \\
       `STRONG_EQUIV y'' E2''` by PROVE_TAC [STRONG_EQUIV_TRANS] \\
-      Q.EXISTS_TAC `E2''` >> ASM_REWRITE_TAC [] \\
-      Q.EXISTS_TAC `y''` >> ASM_REWRITE_TAC [] \\
-      Q.EXISTS_TAC `y'''` >> ASM_REWRITE_TAC [],
+      Q.EXISTS_TAC `E2''` >> art [] \\
+      Q.EXISTS_TAC `y''` >> art [] \\
+      Q.EXISTS_TAC `y'''` >> art [],
       (* goal 2 (of 2) *)
       Q.PAT_X_ASSUM `STRONG_EQUIV y E'`
 	(STRIP_ASSUME_TAC o (ONCE_REWRITE_RULE [PROPERTY_STAR])) \\
@@ -155,9 +152,9 @@ val STRONG_BISIM_UPTO_LEMMA = store_thm (
  ***)
       `STRONG_EQUIV E1'' y'''` by PROVE_TAC [STRONG_EQUIV_TRANS] \\
       `STRONG_EQUIV y'' E2` by PROVE_TAC [STRONG_EQUIV_TRANS] \\
-      Q.EXISTS_TAC `E1''` >> ASM_REWRITE_TAC [] \\
-      Q.EXISTS_TAC `y''` >> ASM_REWRITE_TAC [] \\
-      Q.EXISTS_TAC `y'''` >> ASM_REWRITE_TAC [] ]);
+      Q.EXISTS_TAC `E1''` >> art [] \\
+      Q.EXISTS_TAC `y''` >> art [] \\
+      Q.EXISTS_TAC `y'''` >> art [] ]);
 
 (* To prove (STRONG_EQUIV P Q), we only have to find a weak bisimulation up to STRONG_EQUIV
    which contains (P, Q) *)
@@ -176,8 +173,8 @@ val STRONG_BISIM_UPTO_THM = store_thm (
  >> REWRITE_TAC [RSUBSET, O_DEF]
  >> rpt STRIP_TAC
  >> `STRONG_EQUIV x x /\ STRONG_EQUIV y y` by PROVE_TAC [STRONG_EQUIV_REFL]
- >> Q.EXISTS_TAC `y` >> ASM_REWRITE_TAC []
- >> Q.EXISTS_TAC `x` >> ASM_REWRITE_TAC []);
+ >> Q.EXISTS_TAC `y` >> art []
+ >> Q.EXISTS_TAC `x` >> art []);
 
 (******************************************************************************)
 (*                                                                            *)
@@ -261,85 +258,81 @@ val IDENTITY_WEAK_BISIM_UPTO = store_thm (
       ASSUME_TAC (REWRITE_RULE [ASSUME ``E :('a, 'b) CCS = E'``]
 			       (ASSUME ``TRANS E (label l) E1``)) \\
       IMP_RES_TAC TRANS_IMP_WEAK_TRANS \\
-      Q.EXISTS_TAC `E1` >> ASM_REWRITE_TAC [] \\
+      Q.EXISTS_TAC `E1` >> art [] \\
       REWRITE_TAC [IDENTITY_WEAK_BISIM_UPTO_lemma],
       (* goal 2 (of 4) *)
       IMP_RES_TAC TRANS_IMP_WEAK_TRANS \\
-      Q.EXISTS_TAC `E2` >> ASM_REWRITE_TAC [] \\
+      Q.EXISTS_TAC `E2` >> art [] \\
       REWRITE_TAC [IDENTITY_WEAK_BISIM_UPTO_lemma'],
       (* goal 3 (of 4) *)
       ASSUME_TAC (REWRITE_RULE [ASSUME ``E :('a, 'b) CCS = E'``]
 			       (ASSUME ``TRANS E tau E1``)) \\
       IMP_RES_TAC ONE_TAU \\
-      Q.EXISTS_TAC `E1` >> ASM_REWRITE_TAC [] \\
+      Q.EXISTS_TAC `E1` >> art [] \\
       REWRITE_TAC [IDENTITY_WEAK_BISIM_UPTO_lemma],
       (* goal 4 (of 4) *)
       IMP_RES_TAC ONE_TAU \\
-      Q.EXISTS_TAC `E2` >> ASM_REWRITE_TAC [] \\
+      Q.EXISTS_TAC `E2` >> art [] \\
       REWRITE_TAC [IDENTITY_WEAK_BISIM_UPTO_lemma'] ]);
 
 val CONVERSE_WEAK_BISIM_UPTO_lemma = store_thm (
    "CONVERSE_WEAK_BISIM_UPTO_lemma",
-  ``!Wbsm E E'. (WEAK_EQUIV O (\x y. Wbsm y x) O STRONG_EQUIV) E E' =
+  ``!Wbsm E E'. (WEAK_EQUIV O (inv Wbsm) O STRONG_EQUIV) E E' =
 		(STRONG_EQUIV O Wbsm O WEAK_EQUIV) E' E``,
     rpt GEN_TAC
  >> EQ_TAC (* 2 sub-goals here *)
  >| [ (* goal 1 (of 2) *)
-      REWRITE_TAC [O_DEF] >> BETA_TAC >> rpt STRIP_TAC \\
+      REWRITE_TAC [O_DEF, inv_DEF] >> BETA_TAC >> rpt STRIP_TAC \\
       `STRONG_EQUIV y' E` by PROVE_TAC [STRONG_EQUIV_SYM] \\
       `WEAK_EQUIV E' y` by PROVE_TAC [WEAK_EQUIV_SYM] \\
-      Q.EXISTS_TAC `y'` >> ASM_REWRITE_TAC [] \\
-      Q.EXISTS_TAC `y` >> ASM_REWRITE_TAC [],
+      Q.EXISTS_TAC `y'` >> art [] \\
+      Q.EXISTS_TAC `y` >> art [],
       (* goal 2 (of 2) *)
-      REWRITE_TAC [O_DEF] >> BETA_TAC >> rpt STRIP_TAC \\
+      REWRITE_TAC [O_DEF, inv_DEF] >> BETA_TAC >> rpt STRIP_TAC \\
       `STRONG_EQUIV E y` by PROVE_TAC [STRONG_EQUIV_SYM] \\
       `WEAK_EQUIV y' E'` by PROVE_TAC [WEAK_EQUIV_SYM] \\
-      Q.EXISTS_TAC `y'` >> ASM_REWRITE_TAC [] \\
-      Q.EXISTS_TAC `y` >> ASM_REWRITE_TAC [] ]);
+      Q.EXISTS_TAC `y'` >> art [] \\
+      Q.EXISTS_TAC `y` >> art [] ]);
 
 val CONVERSE_WEAK_BISIM_UPTO_lemma' = store_thm (
    "CONVERSE_WEAK_BISIM_UPTO_lemma'",
-  ``!Wbsm E E'. (STRONG_EQUIV O (\x y. Wbsm y x) O WEAK_EQUIV) E E' =
+  ``!Wbsm E E'. (STRONG_EQUIV O (inv Wbsm) O WEAK_EQUIV) E E' =
 		(WEAK_EQUIV O Wbsm O STRONG_EQUIV) E' E``,
     rpt GEN_TAC
  >> EQ_TAC (* 2 sub-goals here *)
  >| [ (* goal 1 (of 2) *)
-      REWRITE_TAC [O_DEF] >> BETA_TAC >> rpt STRIP_TAC \\
+      REWRITE_TAC [O_DEF, inv_DEF] >> BETA_TAC >> rpt STRIP_TAC \\
       `STRONG_EQUIV E' y` by PROVE_TAC [STRONG_EQUIV_SYM] \\
       `WEAK_EQUIV y' E` by PROVE_TAC [WEAK_EQUIV_SYM] \\
-      Q.EXISTS_TAC `y'` >> ASM_REWRITE_TAC [] \\
-      Q.EXISTS_TAC `y` >> ASM_REWRITE_TAC [],
+      Q.EXISTS_TAC `y'` >> art [] \\
+      Q.EXISTS_TAC `y` >> art [],
       (* goal 2 (of 2) *)
-      REWRITE_TAC [O_DEF] >> BETA_TAC >> rpt STRIP_TAC \\
+      REWRITE_TAC [O_DEF, inv_DEF] >> BETA_TAC >> rpt STRIP_TAC \\
       `STRONG_EQUIV y' E'` by PROVE_TAC [STRONG_EQUIV_SYM] \\
       `WEAK_EQUIV E y` by PROVE_TAC [WEAK_EQUIV_SYM] \\
-      Q.EXISTS_TAC `y'` >> ASM_REWRITE_TAC [] \\
-      Q.EXISTS_TAC `y` >> ASM_REWRITE_TAC [] ]);
+      Q.EXISTS_TAC `y'` >> art [] \\
+      Q.EXISTS_TAC `y` >> art [] ]);
 
 val CONVERSE_WEAK_BISIM_UPTO = store_thm (
    "CONVERSE_WEAK_BISIM_UPTO",
-  ``!Wbsm. WEAK_BISIM_UPTO Wbsm ==> WEAK_BISIM_UPTO (\x y. Wbsm y x)``,
+  ``!Wbsm. WEAK_BISIM_UPTO Wbsm ==> WEAK_BISIM_UPTO (inv Wbsm)``,
     GEN_TAC
  >> PURE_ONCE_REWRITE_TAC [WEAK_BISIM_UPTO]
- >> BETA_TAC
  >> rpt STRIP_TAC
+ >> fs [INVERSE_REL]
  >> RES_TAC (* 4 sub-goals here *)
  >| [ (* goal 1 (of 4) *)
-      Q.EXISTS_TAC `E1'` >> ASM_REWRITE_TAC [] \\
-      REWRITE_TAC [CONVERSE_WEAK_BISIM_UPTO_lemma] \\
-      ASM_REWRITE_TAC [],
+      Q.EXISTS_TAC `E1'` >> art [] \\
+      REWRITE_TAC [CONVERSE_WEAK_BISIM_UPTO_lemma] >> art [],
       (* goal 2 (of 4) *)
-      Q.EXISTS_TAC `E2'` >> ASM_REWRITE_TAC [] \\
-      REWRITE_TAC [CONVERSE_WEAK_BISIM_UPTO_lemma'] \\
-      ASM_REWRITE_TAC [],
+      Q.EXISTS_TAC `E2'` >> art [] \\
+      REWRITE_TAC [CONVERSE_WEAK_BISIM_UPTO_lemma'] >> art [],
       (* goal 3 (of 4) *)
-      Q.EXISTS_TAC `E1'` >> ASM_REWRITE_TAC [] \\
-      REWRITE_TAC [CONVERSE_WEAK_BISIM_UPTO_lemma] \\
-      ASM_REWRITE_TAC [],
+      Q.EXISTS_TAC `E1'` >> art [] \\
+      REWRITE_TAC [CONVERSE_WEAK_BISIM_UPTO_lemma] >> art [],
       (* goal 4 (of 4) *)
-      Q.EXISTS_TAC `E2'` >> ASM_REWRITE_TAC [] \\
-      REWRITE_TAC [CONVERSE_WEAK_BISIM_UPTO_lemma'] \\
-      ASM_REWRITE_TAC [] ]);
+      Q.EXISTS_TAC `E2'` >> art [] \\
+      REWRITE_TAC [CONVERSE_WEAK_BISIM_UPTO_lemma'] >> art [] ]);
 
 val WEAK_BISIM_UPTO_EPS = store_thm ((* NEW *)
    "WEAK_BISIM_UPTO_EPS",
@@ -359,7 +352,7 @@ val WEAK_BISIM_UPTO_EPS = store_thm ((* NEW *)
       RW_TAC std_ss [EPS_REFL] \\
       REWRITE_TAC [O_DEF] >> BETA_TAC \\
       Q.EXISTS_TAC `E'` >> REWRITE_TAC [WEAK_EQUIV_REFL] \\
-      Q.EXISTS_TAC `E` >> ASM_REWRITE_TAC [STRONG_EQUIV_REFL],
+      Q.EXISTS_TAC `E` >> art [STRONG_EQUIV_REFL],
       (* goal 2 (of 2) *)
       RES_TAC \\
       POP_ASSUM (STRIP_ASSUME_TAC o (REWRITE_RULE [O_DEF])) \\
@@ -393,8 +386,8 @@ val WEAK_BISIM_UPTO_EPS = store_thm ((* NEW *)
  *)
       `WEAK_EQUIV y'' E2'''` by PROVE_TAC [WEAK_EQUIV_TRANS] \\
       `STRONG_EQUIV E1' y'''` by PROVE_TAC [STRONG_EQUIV_TRANS] \\
-      Q.EXISTS_TAC `y''` >> ASM_REWRITE_TAC [] \\
-      Q.EXISTS_TAC `y'''` >> ASM_REWRITE_TAC [] ]);
+      Q.EXISTS_TAC `y''` >> art [] \\
+      Q.EXISTS_TAC `y'''` >> art [] ]);
 
 val WEAK_BISIM_UPTO_EPS' = store_thm ((* NEW *)
    "WEAK_BISIM_UPTO_EPS'",
@@ -405,11 +398,11 @@ val WEAK_BISIM_UPTO_EPS' = store_thm ((* NEW *)
  >> POP_ASSUM (ASSUME_TAC o (MATCH_MP CONVERSE_WEAK_BISIM_UPTO))
  >> IMP_RES_TAC WEAK_BISIM_UPTO_EPS
  >> POP_ASSUM MP_TAC
- >> BETA_TAC >> rpt STRIP_TAC
+ >> rpt STRIP_TAC
+ >> IMP_RES_TAC (GSYM INVERSE_REL)
  >> RES_TAC
- >> Q.EXISTS_TAC `E2'` >> ASM_REWRITE_TAC []
- >> REWRITE_TAC [GSYM CONVERSE_WEAK_BISIM_UPTO_lemma]
- >> ASM_REWRITE_TAC []);
+ >> Q.EXISTS_TAC `E2'` >> art []
+ >> REWRITE_TAC [GSYM CONVERSE_WEAK_BISIM_UPTO_lemma] >> art []);
 
 (* Proof sketch:
       E            Wbsm              E'
@@ -440,7 +433,7 @@ val WEAK_BISIM_UPTO_WEAK_TRANS_label = store_thm ((* NEW *)
  >> IMP_RES_TAC (MATCH_MP WEAK_BISIM_UPTO_EPS (* lemma 1 used here *)
 			  (ASSUME ``WEAK_BISIM_UPTO Wbsm``))
  >> POP_ASSUM (STRIP_ASSUME_TAC o (REWRITE_RULE [O_DEF]))
- >> IMP_RES_TAC PROPERTY_STAR_TRANS
+ >> IMP_RES_TAC PROPERTY_STAR_LEFT
  >> IMP_RES_TAC WEAK_BISIM_UPTO_TRANS_label
  >> POP_ASSUM K_TAC
  >> IMP_RES_TAC WEAK_EQUIV_WEAK_TRANS_label
@@ -449,8 +442,8 @@ val WEAK_BISIM_UPTO_WEAK_TRANS_label = store_thm ((* NEW *)
       REWRITE_TAC [O_DEF] >> BETA_TAC >> rpt STRIP_TAC \\
       `STRONG_EQUIV E2 y'''` by PROVE_TAC [STRONG_EQUIV_TRANS] \\
       `WEAK_EQUIV y'' E2''''` by PROVE_TAC [WEAK_EQUIV_TRANS] \\
-      Q.EXISTS_TAC `y''` >> ASM_REWRITE_TAC [] \\
-      Q.EXISTS_TAC `y'''` >> ASM_REWRITE_TAC [] )
+      Q.EXISTS_TAC `y''` >> art [] \\
+      Q.EXISTS_TAC `y'''` >> art [] )
  >> DISCH_TAC
  >> POP_ASSUM (STRIP_ASSUME_TAC o (REWRITE_RULE [O_DEF]))
  >> IMP_RES_TAC (MATCH_MP STRONG_EQUIV_EPS
@@ -466,14 +459,14 @@ val WEAK_BISIM_UPTO_WEAK_TRANS_label = store_thm ((* NEW *)
       REWRITE_TAC [O_DEF] >> BETA_TAC >> rpt STRIP_TAC \\
       `STRONG_EQUIV E1 y'''''` by PROVE_TAC [STRONG_EQUIV_TRANS] \\
       `WEAK_EQUIV y'''' E2'''''''` by PROVE_TAC [WEAK_EQUIV_TRANS] \\
-      Q.EXISTS_TAC `y''''` >> ASM_REWRITE_TAC [] \\
-      Q.EXISTS_TAC `y'''''` >> ASM_REWRITE_TAC [] )
+      Q.EXISTS_TAC `y''''` >> art [] \\
+      Q.EXISTS_TAC `y'''''` >> art [] )
  >> DISCH_TAC
  >> Q.EXISTS_TAC `E2'''''''`
- >> ASM_REWRITE_TAC []
+ >> art []
  >> MATCH_MP_TAC EPS_WEAK_EPS
  >> take [`E2'`, `E2''''`]
- >> ASM_REWRITE_TAC []);
+ >> art []);
 
 val WEAK_BISIM_UPTO_WEAK_TRANS_label' = store_thm ((* NEW *)
    "WEAK_BISIM_UPTO_WEAK_TRANS_label'",
@@ -486,11 +479,11 @@ val WEAK_BISIM_UPTO_WEAK_TRANS_label' = store_thm ((* NEW *)
  >> POP_ASSUM (ASSUME_TAC o (MATCH_MP CONVERSE_WEAK_BISIM_UPTO))
  >> IMP_RES_TAC WEAK_BISIM_UPTO_WEAK_TRANS_label
  >> POP_ASSUM MP_TAC
- >> BETA_TAC >> rpt STRIP_TAC
+ >> rpt STRIP_TAC
+ >> IMP_RES_TAC (GSYM INVERSE_REL)
  >> RES_TAC
- >> Q.EXISTS_TAC `E2'` >> ASM_REWRITE_TAC []
- >> REWRITE_TAC [GSYM CONVERSE_WEAK_BISIM_UPTO_lemma]
- >> ASM_REWRITE_TAC []);
+ >> Q.EXISTS_TAC `E2'` >> art []
+ >> REWRITE_TAC [GSYM CONVERSE_WEAK_BISIM_UPTO_lemma] >> art []);
 
 (* If S is a bisimulation up to WEAK_EQUIV, then (WEAK_EQUIV O S O WEAK_EQUIV) is
    a weak bisimultion. *)
@@ -506,7 +499,7 @@ val WEAK_BISIM_UPTO_LEMMA = store_thm (
 			    (ASSUME ``WEAK_BISIM_UPTO Wbsm``)) \\
       IMP_RES_TAC (MATCH_MP WEAK_EQUIV_WEAK_TRANS_label
 			    (ASSUME ``WEAK_EQUIV y E'``)) \\
-      Q.EXISTS_TAC `E2''` >> ASM_REWRITE_TAC [] \\
+      Q.EXISTS_TAC `E2''` >> art [] \\
       Q.PAT_X_ASSUM `X E2 E2'` (STRIP_ASSUME_TAC o (REWRITE_RULE [O_DEF])) \\
 (***
                E    ~=   y'    Wbsm     y    ~=   E'
@@ -518,15 +511,15 @@ val WEAK_BISIM_UPTO_LEMMA = store_thm (
       `WEAK_EQUIV E2 y'''` by PROVE_TAC [STRONG_IMP_WEAK_EQUIV] \\
       `WEAK_EQUIV E1 y'''` by PROVE_TAC [WEAK_EQUIV_TRANS] \\
       `WEAK_EQUIV y'' E2''` by PROVE_TAC [WEAK_EQUIV_TRANS] \\
-      Q.EXISTS_TAC `y''` >> ASM_REWRITE_TAC [] \\
-      Q.EXISTS_TAC `y'''` >> ASM_REWRITE_TAC [],
+      Q.EXISTS_TAC `y''` >> art [] \\
+      Q.EXISTS_TAC `y'''` >> art [],
       (* goal 2 (of 4) *)
       IMP_RES_TAC (MATCH_MP WEAK_EQUIV_TRANS_label' (ASSUME ``WEAK_EQUIV y E'``)) \\
       IMP_RES_TAC (MATCH_MP WEAK_BISIM_UPTO_WEAK_TRANS_label'
 			    (ASSUME ``WEAK_BISIM_UPTO Wbsm``)) \\
       IMP_RES_TAC (MATCH_MP WEAK_EQUIV_WEAK_TRANS_label'
 			    (ASSUME ``WEAK_EQUIV E y'``)) \\
-      Q.EXISTS_TAC `E1''` >> ASM_REWRITE_TAC [] \\
+      Q.EXISTS_TAC `E1''` >> art [] \\
       Q.PAT_X_ASSUM `X E1' E1` (STRIP_ASSUME_TAC o (REWRITE_RULE [O_DEF])) \\
 (***
                E    ~=     y'      Wbsm    y   ~=   E'
@@ -538,13 +531,13 @@ val WEAK_BISIM_UPTO_LEMMA = store_thm (
       `WEAK_EQUIV E1'' y'''` by PROVE_TAC [WEAK_EQUIV_TRANS] \\
       `WEAK_EQUIV y'' E1` by PROVE_TAC [STRONG_IMP_WEAK_EQUIV] \\
       `WEAK_EQUIV y'' E2` by PROVE_TAC [WEAK_EQUIV_TRANS] \\
-      Q.EXISTS_TAC `y''` >> ASM_REWRITE_TAC [] \\
-      Q.EXISTS_TAC `y'''` >> ASM_REWRITE_TAC [],
+      Q.EXISTS_TAC `y''` >> art [] \\
+      Q.EXISTS_TAC `y'''` >> art [],
       (* goal 3 (of 4) *)
       IMP_RES_TAC (MATCH_MP WEAK_EQUIV_TRANS_tau (ASSUME ``WEAK_EQUIV E y'``)) \\
       IMP_RES_TAC (MATCH_MP WEAK_BISIM_UPTO_EPS (ASSUME ``WEAK_BISIM_UPTO Wbsm``)) \\
       IMP_RES_TAC (MATCH_MP WEAK_EQUIV_EPS (ASSUME ``WEAK_EQUIV y E'``)) \\
-      Q.EXISTS_TAC `E2''` >> ASM_REWRITE_TAC [] \\
+      Q.EXISTS_TAC `E2''` >> art [] \\
       Q.PAT_X_ASSUM `X E2 E2'` (STRIP_ASSUME_TAC o (REWRITE_RULE [O_DEF])) \\
 (***
                E    ~=   y'    Wbsm     y    ~=   E'
@@ -556,13 +549,13 @@ val WEAK_BISIM_UPTO_LEMMA = store_thm (
       `WEAK_EQUIV E2 y'''` by PROVE_TAC [STRONG_IMP_WEAK_EQUIV] \\
       `WEAK_EQUIV E1 y'''` by PROVE_TAC [WEAK_EQUIV_TRANS] \\
       `WEAK_EQUIV y'' E2''` by PROVE_TAC [WEAK_EQUIV_TRANS] \\
-      Q.EXISTS_TAC `y''` >> ASM_REWRITE_TAC [] \\
-      Q.EXISTS_TAC `y'''` >> ASM_REWRITE_TAC [],
+      Q.EXISTS_TAC `y''` >> art [] \\
+      Q.EXISTS_TAC `y'''` >> art [],
       (* goal 4 (of 4) *)
       IMP_RES_TAC (MATCH_MP WEAK_EQUIV_TRANS_tau' (ASSUME ``WEAK_EQUIV y E'``)) \\
       IMP_RES_TAC (MATCH_MP WEAK_BISIM_UPTO_EPS' (ASSUME ``WEAK_BISIM_UPTO Wbsm``)) \\
       IMP_RES_TAC (MATCH_MP WEAK_EQUIV_EPS' (ASSUME ``WEAK_EQUIV E y'``)) \\
-      Q.EXISTS_TAC `E1''` >> ASM_REWRITE_TAC [] \\
+      Q.EXISTS_TAC `E1''` >> art [] \\
       Q.PAT_X_ASSUM `X E1' E1` (STRIP_ASSUME_TAC o (REWRITE_RULE [O_DEF])) \\
 (***
                E    ~=     y'      Wbsm    y   ~=   E'
@@ -574,8 +567,8 @@ val WEAK_BISIM_UPTO_LEMMA = store_thm (
       `WEAK_EQUIV E1'' y'''` by PROVE_TAC [WEAK_EQUIV_TRANS] \\
       `WEAK_EQUIV y'' E1` by PROVE_TAC [STRONG_IMP_WEAK_EQUIV] \\
       `WEAK_EQUIV y'' E2` by PROVE_TAC [WEAK_EQUIV_TRANS] \\
-      Q.EXISTS_TAC `y''` >> ASM_REWRITE_TAC [] \\
-      Q.EXISTS_TAC `y'''` >> ASM_REWRITE_TAC [] ]);
+      Q.EXISTS_TAC `y''` >> art [] \\
+      Q.EXISTS_TAC `y'''` >> art [] ]);
 
 (* To prove (WEAK_EQUIV P Q), we only have to find a weak bisimulation up to WEAK_EQUIV
    which contains (P, Q) *)
@@ -594,8 +587,8 @@ val WEAK_BISIM_UPTO_THM = store_thm (
  >> REWRITE_TAC [RSUBSET, O_DEF]
  >> rpt STRIP_TAC
  >> `WEAK_EQUIV x x /\ WEAK_EQUIV y y` by PROVE_TAC [WEAK_EQUIV_REFL]
- >> Q.EXISTS_TAC `y` >> ASM_REWRITE_TAC []
- >> Q.EXISTS_TAC `x` >> ASM_REWRITE_TAC []);
+ >> Q.EXISTS_TAC `y` >> art []
+ >> Q.EXISTS_TAC `x` >> art []);
 
 (******************************************************************************)
 (*                                                                            *)
@@ -662,7 +655,7 @@ val WEAK_BISIM_UPTO2_EPS = store_thm ((* NEW *)
       Q.EXISTS_TAC `E'` >> REWRITE_TAC [EPS_REFL] \\
       REWRITE_TAC [O_DEF] >> BETA_TAC \\
       Q.EXISTS_TAC `E'` >> REWRITE_TAC [WEAK_EQUIV_REFL] \\
-      Q.EXISTS_TAC `E` >> ASM_REWRITE_TAC [WEAK_EQUIV_REFL],
+      Q.EXISTS_TAC `E` >> art [WEAK_EQUIV_REFL],
       (* goal 2 (of 2) *)
       PROVE_TAC [WEAK_BISIM_UPTO2] ]);
 
@@ -676,7 +669,7 @@ val WEAK_BISIM_UPTO2_EPS' = store_thm ((* NEW *)
  >| [ (* goal 1 (of 2) *)
       Q.EXISTS_TAC `E` >> REWRITE_TAC [EPS_REFL] \\
       REWRITE_TAC [O_DEF] >> BETA_TAC \\
-      Q.EXISTS_TAC `E'` >> ASM_REWRITE_TAC [WEAK_EQUIV_REFL] \\
+      Q.EXISTS_TAC `E'` >> art [WEAK_EQUIV_REFL] \\
       Q.EXISTS_TAC `E` >> REWRITE_TAC [WEAK_EQUIV_REFL] \\
       PROVE_TAC [],
       (* goal 2 (of 2) *)
@@ -696,7 +689,7 @@ val WEAK_BISIM_UPTO2_LEMMA = store_thm (
 			    (ASSUME ``WEAK_BISIM_UPTO2 Wbsm``)) \\
       IMP_RES_TAC (MATCH_MP WEAK_EQUIV_WEAK_TRANS_label
 			    (ASSUME ``WEAK_EQUIV y E'``)) \\
-      Q.EXISTS_TAC `E2''` >> ASM_REWRITE_TAC [] \\
+      Q.EXISTS_TAC `E2''` >> art [] \\
       Q.PAT_X_ASSUM `X E2 E2'` (STRIP_ASSUME_TAC o (REWRITE_RULE [O_DEF])) \\
 (***
                E    ~=   y'     Wbsm     y    ~=   E'
@@ -707,15 +700,15 @@ val WEAK_BISIM_UPTO2_LEMMA = store_thm (
  ***)
       `WEAK_EQUIV E1 y'''` by PROVE_TAC [WEAK_EQUIV_TRANS] \\
       `WEAK_EQUIV y'' E2''` by PROVE_TAC [WEAK_EQUIV_TRANS] \\
-      Q.EXISTS_TAC `y''` >> ASM_REWRITE_TAC [] \\
-      Q.EXISTS_TAC `y'''` >> ASM_REWRITE_TAC [],
+      Q.EXISTS_TAC `y''` >> art [] \\
+      Q.EXISTS_TAC `y'''` >> art [],
       (* goal 2 (of 4) *)
       IMP_RES_TAC (MATCH_MP WEAK_EQUIV_TRANS_label' (ASSUME ``WEAK_EQUIV y E'``)) \\
       IMP_RES_TAC (MATCH_MP WEAK_BISIM_UPTO2_WEAK_TRANS_label'
 			    (ASSUME ``WEAK_BISIM_UPTO2 Wbsm``)) \\
       IMP_RES_TAC (MATCH_MP WEAK_EQUIV_WEAK_TRANS_label'
 			    (ASSUME ``WEAK_EQUIV E y'``)) \\
-      Q.EXISTS_TAC `E1''` >> ASM_REWRITE_TAC [] \\
+      Q.EXISTS_TAC `E1''` >> art [] \\
       Q.PAT_X_ASSUM `X E1' E1` (STRIP_ASSUME_TAC o (REWRITE_RULE [O_DEF])) \\
 (***
                E    ~=     y'      Wbsm    y   ~=   E'
@@ -726,13 +719,13 @@ val WEAK_BISIM_UPTO2_LEMMA = store_thm (
  ***)
       `WEAK_EQUIV E1'' y'''` by PROVE_TAC [WEAK_EQUIV_TRANS] \\
       `WEAK_EQUIV y'' E2` by PROVE_TAC [WEAK_EQUIV_TRANS] \\
-      Q.EXISTS_TAC `y''` >> ASM_REWRITE_TAC [] \\
-      Q.EXISTS_TAC `y'''` >> ASM_REWRITE_TAC [],
+      Q.EXISTS_TAC `y''` >> art [] \\
+      Q.EXISTS_TAC `y'''` >> art [],
       (* goal 3 (of 4) *)
       IMP_RES_TAC (MATCH_MP WEAK_EQUIV_TRANS_tau (ASSUME ``WEAK_EQUIV E y'``)) \\
       IMP_RES_TAC (MATCH_MP WEAK_BISIM_UPTO2_EPS (ASSUME ``WEAK_BISIM_UPTO2 Wbsm``)) \\
       IMP_RES_TAC (MATCH_MP WEAK_EQUIV_EPS (ASSUME ``WEAK_EQUIV y E'``)) \\
-      Q.EXISTS_TAC `E2''` >> ASM_REWRITE_TAC [] \\
+      Q.EXISTS_TAC `E2''` >> art [] \\
       Q.PAT_X_ASSUM `X E2 E2'` (STRIP_ASSUME_TAC o (REWRITE_RULE [O_DEF])) \\
 (***
                E    ~=   y'    Wbsm     y    ~=   E'
@@ -743,13 +736,13 @@ val WEAK_BISIM_UPTO2_LEMMA = store_thm (
  ***)
       `WEAK_EQUIV E1 y'''` by PROVE_TAC [WEAK_EQUIV_TRANS] \\
       `WEAK_EQUIV y'' E2''` by PROVE_TAC [WEAK_EQUIV_TRANS] \\
-      Q.EXISTS_TAC `y''` >> ASM_REWRITE_TAC [] \\
-      Q.EXISTS_TAC `y'''` >> ASM_REWRITE_TAC [],
+      Q.EXISTS_TAC `y''` >> art [] \\
+      Q.EXISTS_TAC `y'''` >> art [],
       (* goal 4 (of 4) *)
       IMP_RES_TAC (MATCH_MP WEAK_EQUIV_TRANS_tau' (ASSUME ``WEAK_EQUIV y E'``)) \\
       IMP_RES_TAC (MATCH_MP WEAK_BISIM_UPTO2_EPS' (ASSUME ``WEAK_BISIM_UPTO2 Wbsm``)) \\
       IMP_RES_TAC (MATCH_MP WEAK_EQUIV_EPS' (ASSUME ``WEAK_EQUIV E y'``)) \\
-      Q.EXISTS_TAC `E1''` >> ASM_REWRITE_TAC [] \\
+      Q.EXISTS_TAC `E1''` >> art [] \\
       Q.PAT_X_ASSUM `X E1' E1` (STRIP_ASSUME_TAC o (REWRITE_RULE [O_DEF])) \\
 (***
                E    ~=     y'      Wbsm    y   ~=   E'
@@ -760,8 +753,8 @@ val WEAK_BISIM_UPTO2_LEMMA = store_thm (
  ***)
       `WEAK_EQUIV E1'' y'''` by PROVE_TAC [WEAK_EQUIV_TRANS] \\
       `WEAK_EQUIV y'' E2` by PROVE_TAC [WEAK_EQUIV_TRANS] \\
-      Q.EXISTS_TAC `y''` >> ASM_REWRITE_TAC [] \\
-      Q.EXISTS_TAC `y'''` >> ASM_REWRITE_TAC [] ]);
+      Q.EXISTS_TAC `y''` >> art [] \\
+      Q.EXISTS_TAC `y'''` >> art [] ]);
 
 (* To prove (WEAK_EQUIV P Q), we only have to find a weak bisimulation up to WEAK_EQUIV
    which contains (P, Q) *)
@@ -780,8 +773,8 @@ val WEAK_BISIM_UPTO2_THM = store_thm (
  >> REWRITE_TAC [RSUBSET, O_DEF]
  >> rpt STRIP_TAC
  >> `WEAK_EQUIV x x /\ WEAK_EQUIV y y` by PROVE_TAC [WEAK_EQUIV_REFL]
- >> Q.EXISTS_TAC `y` >> ASM_REWRITE_TAC []
- >> Q.EXISTS_TAC `x` >> ASM_REWRITE_TAC []);
+ >> Q.EXISTS_TAC `y` >> art []
+ >> Q.EXISTS_TAC `x` >> art []);
 
 (******************************************************************************)
 (*                                                                            *)
@@ -823,29 +816,27 @@ val IDENTITY_OBS_BISIM_UPTO = store_thm (
       ASSUME_TAC (REWRITE_RULE [ASSUME ``E :('a, 'b) CCS = E'``]
 			       (ASSUME ``TRANS E u E1``)) \\
       IMP_RES_TAC TRANS_IMP_WEAK_TRANS \\
-      Q.EXISTS_TAC `E1` >> ASM_REWRITE_TAC [] \\
+      Q.EXISTS_TAC `E1` >> art [] \\
       REWRITE_TAC [IDENTITY_WEAK_BISIM_UPTO_lemma],
       (* goal 2 (of 4) *)
       IMP_RES_TAC TRANS_IMP_WEAK_TRANS \\
-      Q.EXISTS_TAC `E2` >> ASM_REWRITE_TAC [] \\
+      Q.EXISTS_TAC `E2` >> art [] \\
       REWRITE_TAC [IDENTITY_WEAK_BISIM_UPTO_lemma'] ]);
 
 val CONVERSE_OBS_BISIM_UPTO = store_thm (
    "CONVERSE_OBS_BISIM_UPTO",
-  ``!Obsm. OBS_BISIM_UPTO Obsm ==> OBS_BISIM_UPTO (\x y. Obsm y x)``,
+  ``!Obsm. OBS_BISIM_UPTO Obsm ==> OBS_BISIM_UPTO (inv Obsm)``,
     GEN_TAC
  >> PURE_ONCE_REWRITE_TAC [OBS_BISIM_UPTO]
- >> BETA_TAC
  >> rpt STRIP_TAC
+ >> IMP_RES_TAC (GSYM INVERSE_REL)
  >> RES_TAC (* 2 sub-goals here *)
  >| [ (* goal 1 (of 2) *)
-      Q.EXISTS_TAC `E1'` >> ASM_REWRITE_TAC [] \\
-      REWRITE_TAC [CONVERSE_WEAK_BISIM_UPTO_lemma] \\
-      ASM_REWRITE_TAC [],
+      Q.EXISTS_TAC `E1'` >> art [] \\
+      REWRITE_TAC [CONVERSE_WEAK_BISIM_UPTO_lemma] >> art [],
       (* goal 2 (of 2) *)
-      Q.EXISTS_TAC `E2'` >> ASM_REWRITE_TAC [] \\
-      REWRITE_TAC [CONVERSE_WEAK_BISIM_UPTO_lemma'] \\
-      ASM_REWRITE_TAC [] ]);
+      Q.EXISTS_TAC `E2'` >> art [] \\
+      REWRITE_TAC [CONVERSE_WEAK_BISIM_UPTO_lemma'] >> art [] ]);
 
 val OBS_BISIM_UPTO_EPS = store_thm ((* NEW *)
    "OBS_BISIM_UPTO_EPS",
@@ -865,11 +856,11 @@ val OBS_BISIM_UPTO_EPS = store_thm ((* NEW *)
       RW_TAC std_ss [EPS_REFL] \\
       REWRITE_TAC [O_DEF] >> BETA_TAC \\
       Q.EXISTS_TAC `E'` >> REWRITE_TAC [WEAK_EQUIV_REFL] \\
-      Q.EXISTS_TAC `E` >> ASM_REWRITE_TAC [STRONG_EQUIV_REFL],
+      Q.EXISTS_TAC `E` >> art [STRONG_EQUIV_REFL],
       (* goal 2 (of 2) *)
       RES_TAC \\
       POP_ASSUM (STRIP_ASSUME_TAC o (REWRITE_RULE [O_DEF])) \\
-      IMP_RES_TAC PROPERTY_STAR_TRANS \\
+      IMP_RES_TAC PROPERTY_STAR_LEFT \\
       IMP_RES_TAC OBS_BISIM_UPTO_TRANS \\
       IMP_RES_TAC WEAK_EQUIV_WEAK_TRANS_tau \\
       Q.EXISTS_TAC `E2'''` \\
@@ -889,8 +880,8 @@ val OBS_BISIM_UPTO_EPS = store_thm ((* NEW *)
  *)
       `WEAK_EQUIV y'' E2'''` by PROVE_TAC [WEAK_EQUIV_TRANS] \\
       `STRONG_EQUIV E1' y'''` by PROVE_TAC [STRONG_EQUIV_TRANS] \\
-      Q.EXISTS_TAC `y''` >> ASM_REWRITE_TAC [] \\
-      Q.EXISTS_TAC `y'''` >> ASM_REWRITE_TAC [] ]);
+      Q.EXISTS_TAC `y''` >> art [] \\
+      Q.EXISTS_TAC `y'''` >> art [] ]);
 
 val OBS_BISIM_UPTO_EPS' = store_thm ((* NEW *)
    "OBS_BISIM_UPTO_EPS'",
@@ -901,11 +892,11 @@ val OBS_BISIM_UPTO_EPS' = store_thm ((* NEW *)
  >> POP_ASSUM (ASSUME_TAC o (MATCH_MP CONVERSE_OBS_BISIM_UPTO))
  >> IMP_RES_TAC OBS_BISIM_UPTO_EPS
  >> POP_ASSUM MP_TAC
- >> BETA_TAC >> rpt STRIP_TAC
+ >> rpt STRIP_TAC
+ >> IMP_RES_TAC INVERSE_REL
  >> RES_TAC
- >> Q.EXISTS_TAC `E2'` >> ASM_REWRITE_TAC []
- >> REWRITE_TAC [GSYM CONVERSE_WEAK_BISIM_UPTO_lemma]
- >> ASM_REWRITE_TAC []);
+ >> Q.EXISTS_TAC `E2'` >> art []
+ >> REWRITE_TAC [GSYM CONVERSE_WEAK_BISIM_UPTO_lemma] >> art []);
 
 (* Proof sketch:
       E            Obsm              E'
@@ -936,7 +927,7 @@ val OBS_BISIM_UPTO_WEAK_TRANS_label = store_thm ((* NEW *)
  >> IMP_RES_TAC (MATCH_MP OBS_BISIM_UPTO_EPS (* lemma 1 used here *)
 			  (ASSUME ``OBS_BISIM_UPTO Obsm``))
  >> POP_ASSUM (STRIP_ASSUME_TAC o (REWRITE_RULE [O_DEF]))
- >> IMP_RES_TAC PROPERTY_STAR_TRANS
+ >> IMP_RES_TAC PROPERTY_STAR_LEFT
  >> IMP_RES_TAC OBS_BISIM_UPTO_TRANS
  >> POP_ASSUM K_TAC
  >> IMP_RES_TAC WEAK_EQUIV_WEAK_TRANS_label
@@ -945,8 +936,8 @@ val OBS_BISIM_UPTO_WEAK_TRANS_label = store_thm ((* NEW *)
       REWRITE_TAC [O_DEF] >> BETA_TAC >> rpt STRIP_TAC \\
       `STRONG_EQUIV E2 y'''` by PROVE_TAC [STRONG_EQUIV_TRANS] \\
       `WEAK_EQUIV y'' E2''''` by PROVE_TAC [WEAK_EQUIV_TRANS] \\
-      Q.EXISTS_TAC `y''` >> ASM_REWRITE_TAC [] \\
-      Q.EXISTS_TAC `y'''` >> ASM_REWRITE_TAC [] )
+      Q.EXISTS_TAC `y''` >> art [] \\
+      Q.EXISTS_TAC `y'''` >> art [] )
  >> DISCH_TAC
  >> POP_ASSUM (STRIP_ASSUME_TAC o (REWRITE_RULE [O_DEF]))
  >> IMP_RES_TAC (MATCH_MP STRONG_EQUIV_EPS
@@ -962,14 +953,14 @@ val OBS_BISIM_UPTO_WEAK_TRANS_label = store_thm ((* NEW *)
       REWRITE_TAC [O_DEF] >> BETA_TAC >> rpt STRIP_TAC \\
       `STRONG_EQUIV E1 y'''''` by PROVE_TAC [STRONG_EQUIV_TRANS] \\
       `WEAK_EQUIV y'''' E2'''''''` by PROVE_TAC [WEAK_EQUIV_TRANS] \\
-      Q.EXISTS_TAC `y''''` >> ASM_REWRITE_TAC [] \\
-      Q.EXISTS_TAC `y'''''` >> ASM_REWRITE_TAC [] )
+      Q.EXISTS_TAC `y''''` >> art [] \\
+      Q.EXISTS_TAC `y'''''` >> art [] )
  >> DISCH_TAC
  >> Q.EXISTS_TAC `E2'''''''`
- >> ASM_REWRITE_TAC []
+ >> art []
  >> MATCH_MP_TAC EPS_WEAK_EPS
  >> take [`E2'`, `E2''''`]
- >> ASM_REWRITE_TAC []);
+ >> art []);
 
 val OBS_BISIM_UPTO_WEAK_TRANS_label' = store_thm ((* NEW *)
    "OBS_BISIM_UPTO_WEAK_TRANS_label'",
@@ -982,11 +973,11 @@ val OBS_BISIM_UPTO_WEAK_TRANS_label' = store_thm ((* NEW *)
  >> POP_ASSUM (ASSUME_TAC o (MATCH_MP CONVERSE_OBS_BISIM_UPTO))
  >> IMP_RES_TAC OBS_BISIM_UPTO_WEAK_TRANS_label
  >> POP_ASSUM MP_TAC
- >> BETA_TAC >> rpt STRIP_TAC
+ >> rpt STRIP_TAC
+ >> IMP_RES_TAC INVERSE_REL
  >> RES_TAC
- >> Q.EXISTS_TAC `E2'` >> ASM_REWRITE_TAC []
- >> REWRITE_TAC [GSYM CONVERSE_WEAK_BISIM_UPTO_lemma]
- >> ASM_REWRITE_TAC []);
+ >> Q.EXISTS_TAC `E2'` >> art []
+ >> REWRITE_TAC [GSYM CONVERSE_WEAK_BISIM_UPTO_lemma] >> art []);
 
 (* To prove (OBS_CONGR P Q), we only have to find a `Obs` bisimulation up to WEAK_EQUIV
    which contains (P, Q) *)
@@ -1002,13 +993,13 @@ val OBS_BISIM_UPTO_THM = store_thm (
  >> rpt STRIP_TAC (* 2 sub-goals here *)
  >| [ (* goal 1 (of 2) *)
       RES_TAC \\
-      Q.EXISTS_TAC `E2` >> ASM_REWRITE_TAC [] \\
+      Q.EXISTS_TAC `E2` >> art [] \\
       irule (REWRITE_RULE [RSUBSET] WEAK_BISIM_UPTO_THM) \\
-      Q.EXISTS_TAC `(WEAK_EQUIV O Obsm O STRONG_EQUIV)` >> ASM_REWRITE_TAC [] \\
+      Q.EXISTS_TAC `(WEAK_EQUIV O Obsm O STRONG_EQUIV)` >> art [] \\
       REWRITE_TAC [WEAK_BISIM_UPTO] >> rpt STRIP_TAC >| (* 4 sub-goals here *)
       [ (* goal 1.1 (of 4) *)
         Q.PAT_X_ASSUM `X E E'` (STRIP_ASSUME_TAC o BETA_RULE o (REWRITE_RULE [O_DEF])) \\
-        IMP_RES_TAC PROPERTY_STAR_TRANS \\
+        IMP_RES_TAC PROPERTY_STAR_LEFT \\
         Q.PAT_X_ASSUM `Obsm x y` K_TAC \\
         IMP_RES_TAC OBS_BISIM_UPTO_TRANS \\
         Q.PAT_X_ASSUM `WEAK_TRANS y u E2` K_TAC \\
@@ -1020,10 +1011,10 @@ val OBS_BISIM_UPTO_THM = store_thm (
 	|        |               ||        ||
        !E1'  ~   E2' (~ Obsm ~~) E2'' ~~  E2'''
  ***)
-        Q.EXISTS_TAC `E2'''` >> ASM_REWRITE_TAC [] \\
+        Q.EXISTS_TAC `E2'''` >> art [] \\
         NTAC 2 (ONCE_REWRITE_TAC [O_DEF]) \\
-        Q.EXISTS_TAC `E2''` >> ASM_REWRITE_TAC [] \\
-        Q.EXISTS_TAC `E2'` >> ASM_REWRITE_TAC [],
+        Q.EXISTS_TAC `E2''` >> art [] \\
+        Q.EXISTS_TAC `E2'` >> art [],
         (* goal 1.2 (of 4) *)
         Q.PAT_X_ASSUM `X E E'` (STRIP_ASSUME_TAC o BETA_RULE o (REWRITE_RULE [O_DEF])) \\
         IMP_RES_TAC WEAK_EQUIV_TRANS_label' \\
@@ -1037,19 +1028,19 @@ val OBS_BISIM_UPTO_THM = store_thm (
 	||       ||                        ||        |
 	E1''' ~  E1'' ~ y'''' Obsm y''' ~~ E1'  ~~  !E2'
  ***)
-        Q.EXISTS_TAC `E1'''` >> ASM_REWRITE_TAC [] \\
+        Q.EXISTS_TAC `E1'''` >> art [] \\
         Q.PAT_X_ASSUM `X E1'' E1'` MP_TAC \\
         REWRITE_TAC [O_DEF] >> BETA_TAC >> rpt STRIP_TAC \\
         IMP_RES_TAC STRONG_IMP_WEAK_EQUIV \\
         `WEAK_EQUIV E1''' y''''` by PROVE_TAC [WEAK_EQUIV_TRANS] \\
         `WEAK_EQUIV y''' E2'`  by PROVE_TAC [WEAK_EQUIV_TRANS] \\
         Q.EXISTS_TAC `E2'` >> REWRITE_TAC [STRONG_EQUIV_REFL] \\
-        Q.EXISTS_TAC `y''''` >> ASM_REWRITE_TAC [] \\
-        Q.EXISTS_TAC `y'''` >> ASM_REWRITE_TAC [] \\
-        Q.EXISTS_TAC `y''''` >> ASM_REWRITE_TAC [STRONG_EQUIV_REFL],
+        Q.EXISTS_TAC `y''''` >> art [] \\
+        Q.EXISTS_TAC `y'''` >> art [] \\
+        Q.EXISTS_TAC `y''''` >> art [STRONG_EQUIV_REFL],
         (* goal 1.3 (of 4) *)
         Q.PAT_X_ASSUM `X E E'` (STRIP_ASSUME_TAC o BETA_RULE o (REWRITE_RULE [O_DEF])) \\
-        IMP_RES_TAC PROPERTY_STAR_TRANS \\
+        IMP_RES_TAC PROPERTY_STAR_LEFT \\
         Q.PAT_X_ASSUM `Obsm x y` K_TAC \\
         IMP_RES_TAC OBS_BISIM_UPTO_TRANS \\
         Q.PAT_X_ASSUM `WEAK_TRANS y u E2` K_TAC \\
@@ -1061,10 +1052,10 @@ val OBS_BISIM_UPTO_THM = store_thm (
 	|        |               ||        ||
        !E1'  ~   E2' (~ Obsm ~~) E2'' ~~  E2'''
  ***)
-        Q.EXISTS_TAC `E2'''` >> ASM_REWRITE_TAC [] \\
+        Q.EXISTS_TAC `E2'''` >> art [] \\
         NTAC 2 (ONCE_REWRITE_TAC [O_DEF]) \\
-        Q.EXISTS_TAC `E2''` >> ASM_REWRITE_TAC [] \\
-        Q.EXISTS_TAC `E2'` >> ASM_REWRITE_TAC [],
+        Q.EXISTS_TAC `E2''` >> art [] \\
+        Q.EXISTS_TAC `E2'` >> art [],
         (* goal 1.4 (of 4) *)
         Q.PAT_X_ASSUM `X E E'` (STRIP_ASSUME_TAC o BETA_RULE o (REWRITE_RULE [O_DEF])) \\
         IMP_RES_TAC WEAK_EQUIV_TRANS_tau' \\
@@ -1078,21 +1069,21 @@ val OBS_BISIM_UPTO_THM = store_thm (
 	||       ||                        ||        |
 	E1''' ~  E1'' ~ y'''' Obsm y''' ~~ E1'  ~~  !E2'
  ***)
-        Q.EXISTS_TAC `E1'''` >> ASM_REWRITE_TAC [] \\
+        Q.EXISTS_TAC `E1'''` >> art [] \\
         Q.PAT_X_ASSUM `X E1'' E1'` MP_TAC \\
         REWRITE_TAC [O_DEF] >> BETA_TAC >> rpt STRIP_TAC \\
         IMP_RES_TAC STRONG_IMP_WEAK_EQUIV \\
         `WEAK_EQUIV E1''' y''''` by PROVE_TAC [WEAK_EQUIV_TRANS] \\
         `WEAK_EQUIV y''' E2'`  by PROVE_TAC [WEAK_EQUIV_TRANS] \\
         Q.EXISTS_TAC `E2'` >> REWRITE_TAC [STRONG_EQUIV_REFL] \\
-        Q.EXISTS_TAC `y''''` >> ASM_REWRITE_TAC [] \\
-        Q.EXISTS_TAC `y'''` >> ASM_REWRITE_TAC [] \\
-        Q.EXISTS_TAC `y''''` >> ASM_REWRITE_TAC [STRONG_EQUIV_REFL] ],
+        Q.EXISTS_TAC `y''''` >> art [] \\
+        Q.EXISTS_TAC `y'''` >> art [] \\
+        Q.EXISTS_TAC `y''''` >> art [STRONG_EQUIV_REFL] ],
       (* goal 2 (of 2) *)
       RES_TAC \\
-      Q.EXISTS_TAC `E1` >> ASM_REWRITE_TAC [] \\
+      Q.EXISTS_TAC `E1` >> art [] \\
       irule (REWRITE_RULE [RSUBSET] WEAK_BISIM_UPTO_THM) \\
-      Q.EXISTS_TAC `(STRONG_EQUIV O Obsm O WEAK_EQUIV)` >> ASM_REWRITE_TAC [] \\
+      Q.EXISTS_TAC `(STRONG_EQUIV O Obsm O WEAK_EQUIV)` >> art [] \\
       REWRITE_TAC [WEAK_BISIM_UPTO] >> rpt STRIP_TAC >| (* 4 sub-goals here *)
       [ (* goal 2.1 (of 4) *)
         Q.PAT_X_ASSUM `X E E'` (STRIP_ASSUME_TAC o BETA_RULE o (REWRITE_RULE [O_DEF])) \\
@@ -1108,19 +1099,19 @@ val OBS_BISIM_UPTO_THM = store_thm (
 	|        ||              ||        ||
        !E1'  ~~  E2' (~ Obsm ~~) E2'' ~   E2'''
  ***)
-        Q.EXISTS_TAC `E2'''` >> ASM_REWRITE_TAC [] \\
+        Q.EXISTS_TAC `E2'''` >> art [] \\
         Q.PAT_X_ASSUM `X E2' E2''` MP_TAC \\
         REWRITE_TAC [O_DEF] >> BETA_TAC >> rpt STRIP_TAC \\
         IMP_RES_TAC STRONG_IMP_WEAK_EQUIV \\
         `WEAK_EQUIV E1' y''''` by PROVE_TAC [WEAK_EQUIV_TRANS] \\
         `WEAK_EQUIV y''' E2'''`  by PROVE_TAC [WEAK_EQUIV_TRANS] \\
-        Q.EXISTS_TAC `y'''` >> ASM_REWRITE_TAC [] \\
+        Q.EXISTS_TAC `y'''` >> art [] \\
         Q.EXISTS_TAC `E1'` >> REWRITE_TAC [STRONG_EQUIV_REFL] \\
         Q.EXISTS_TAC `y'''` >> REWRITE_TAC [STRONG_EQUIV_REFL] \\
-        Q.EXISTS_TAC `y''''` >> ASM_REWRITE_TAC [],
+        Q.EXISTS_TAC `y''''` >> art [],
         (* goal 2.2 (of 4) *)
         Q.PAT_X_ASSUM `X E E'` (STRIP_ASSUME_TAC o BETA_RULE o (REWRITE_RULE [O_DEF])) \\
-        IMP_RES_TAC PROPERTY_STAR_TRANS' \\
+        IMP_RES_TAC PROPERTY_STAR_RIGHT \\
         Q.PAT_X_ASSUM `Obsm x y` K_TAC \\
         IMP_RES_TAC OBS_BISIM_UPTO_TRANS' \\
         IMP_RES_TAC WEAK_EQUIV_WEAK_TRANS_label' \\
@@ -1131,10 +1122,10 @@ val OBS_BISIM_UPTO_THM = store_thm (
 	||       ||                        |        |
 	E1''' ~~ E1'' ~ y'''' Obsm y''' ~~ E1'  ~  !E2'
  ***)
-        Q.EXISTS_TAC `E1'''` >> ASM_REWRITE_TAC [] \\
+        Q.EXISTS_TAC `E1'''` >> art [] \\
         NTAC 2 (ONCE_REWRITE_TAC [O_DEF]) \\
-        Q.EXISTS_TAC `E1'` >> ASM_REWRITE_TAC [] \\
-        Q.EXISTS_TAC `E1''` >> ASM_REWRITE_TAC [],
+        Q.EXISTS_TAC `E1'` >> art [] \\
+        Q.EXISTS_TAC `E1''` >> art [],
         (* goal 2.3 (of 4) *)
         Q.PAT_X_ASSUM `X E E'` (STRIP_ASSUME_TAC o BETA_RULE o (REWRITE_RULE [O_DEF])) \\
         IMP_RES_TAC WEAK_EQUIV_TRANS_tau \\
@@ -1149,19 +1140,19 @@ val OBS_BISIM_UPTO_THM = store_thm (
 	|        ||              ||        ||
        !E1'  ~~  E2' (~ Obsm ~~) E2'' ~   E2'''
  ***)
-        Q.EXISTS_TAC `E2'''` >> ASM_REWRITE_TAC [] \\
+        Q.EXISTS_TAC `E2'''` >> art [] \\
         Q.PAT_X_ASSUM `X E2' E2''` MP_TAC \\
         REWRITE_TAC [O_DEF] >> BETA_TAC >> rpt STRIP_TAC \\
         IMP_RES_TAC STRONG_IMP_WEAK_EQUIV \\
         `WEAK_EQUIV E1' y''''` by PROVE_TAC [WEAK_EQUIV_TRANS] \\
         `WEAK_EQUIV y''' E2'''`  by PROVE_TAC [WEAK_EQUIV_TRANS] \\
-        Q.EXISTS_TAC `y'''` >> ASM_REWRITE_TAC [] \\
+        Q.EXISTS_TAC `y'''` >> art [] \\
         Q.EXISTS_TAC `E1'` >> REWRITE_TAC [STRONG_EQUIV_REFL] \\
         Q.EXISTS_TAC `y'''` >> REWRITE_TAC [STRONG_EQUIV_REFL] \\
-        Q.EXISTS_TAC `y''''` >> ASM_REWRITE_TAC [],
+        Q.EXISTS_TAC `y''''` >> art [],
         (* goal 2.4 (of 4) *)
         Q.PAT_X_ASSUM `X E E'` (STRIP_ASSUME_TAC o BETA_RULE o (REWRITE_RULE [O_DEF])) \\
-        IMP_RES_TAC PROPERTY_STAR_TRANS' \\
+        IMP_RES_TAC PROPERTY_STAR_RIGHT \\
         Q.PAT_X_ASSUM `Obsm x y` K_TAC \\
         IMP_RES_TAC OBS_BISIM_UPTO_TRANS' \\
         IMP_RES_TAC WEAK_EQUIV_WEAK_TRANS_tau' \\
@@ -1172,10 +1163,10 @@ val OBS_BISIM_UPTO_THM = store_thm (
 	||       ||                        |        |
 	E1''' ~~ E1'' ~ y'''' Obsm y''' ~~ E1'  ~  !E2'
  ***)
-        Q.EXISTS_TAC `E1'''` >> ASM_REWRITE_TAC [] \\
+        Q.EXISTS_TAC `E1'''` >> art [] \\
         NTAC 2 (ONCE_REWRITE_TAC [O_DEF]) \\
-        Q.EXISTS_TAC `E1'` >> ASM_REWRITE_TAC [] \\
-        Q.EXISTS_TAC `E1''` >> ASM_REWRITE_TAC [] ] ]);
+        Q.EXISTS_TAC `E1'` >> art [] \\
+        Q.EXISTS_TAC `E1''` >> art [] ] ]);
 
 (* Bibliography:
  *
