thesis/CoarsestCongrScript.sml
@@ -10,7 +10,8 @@ open prim_recTheory arithmeticTheory combinTheory;
 open cardinalTheory ordinalTheory;
 
 open CCSLib CCSTheory GraphTheory;
-open StrongEQTheory StrongLawsTheory WeakEQTheory WeakLawsTheory;
+open StrongEQTheory StrongEQLib StrongLawsTheory;
+open WeakEQTheory WeakEQLib WeakLawsTheory;
 open ObsCongrTheory ObsCongrLib ObsCongrLawsTheory ObsCongrConv;
 open TraceTheory CongruenceTheory;
 
@@ -29,7 +30,7 @@ val _ = temp_loose_equality ();
 val TAU_STRAT = store_thm (
    "TAU_STRAT",
   ``!E E'. OBS_CONGR (sum E (prefix tau (sum E' E))) (prefix tau (sum E' E))``,
-    REPEAT GEN_TAC
+    rpt GEN_TAC
  >> OC_LHS_SUBST1_TAC
        (SPEC ``sum E' E`` (GEN_ALL (OC_SYM (SPEC_ALL TAU2))))
  >> OC_SUM_IDEMP_TAC
@@ -47,16 +48,16 @@ val DENG_LEMMA = store_thm ((* NEW *)
   ``!p q. WEAK_EQUIV p q ==> (?p'. TRANS p tau p' /\ WEAK_EQUIV p' q) \/
 			     (?q'. TRANS q tau q' /\ WEAK_EQUIV p q') \/
 			     OBS_CONGR p q``,
-    REPEAT STRIP_TAC
+    rpt STRIP_TAC
  >> MATCH_MP_TAC (DECIDE ``(~P /\ ~Q ==> R) ==> P \/ Q \/ R``)
- >> REPEAT STRIP_TAC
+ >> rpt STRIP_TAC
  >> REWRITE_TAC [OBS_CONGR]
- >> REPEAT STRIP_TAC (* 2 sub-goals here *)
+ >> rpt STRIP_TAC (* 2 sub-goals here *)
  >| [ (* goal 1 (of 2) *)
       Cases_on `u` >| (* 2 sub-goals here *)
       [ (* goal 1.1 (of 2) *)
         PAT_X_ASSUM ``WEAK_EQUIV p q``
-		(STRIP_ASSUME_TAC o (ONCE_REWRITE_RULE [OBS_PROPERTY_STAR])) \\
+		(STRIP_ASSUME_TAC o (ONCE_REWRITE_RULE [WEAK_PROPERTY_STAR])) \\
         RES_TAC \\
         IMP_RES_TAC EPS_cases1 >- PROVE_TAC [] \\
         Q.EXISTS_TAC `E2` >> ASM_REWRITE_TAC [] \\
@@ -64,14 +65,14 @@ val DENG_LEMMA = store_thm ((* NEW *)
         take [`q`, `u`] >> ASM_REWRITE_TAC [EPS_REFL, PREFIX],
         (* goal 1.2 (of 2) *)
         PAT_X_ASSUM ``WEAK_EQUIV p q``
-		(STRIP_ASSUME_TAC o (ONCE_REWRITE_RULE [OBS_PROPERTY_STAR])) \\
+		(STRIP_ASSUME_TAC o (ONCE_REWRITE_RULE [WEAK_PROPERTY_STAR])) \\
         RES_TAC \\
         Q.EXISTS_TAC `E2` >> ASM_REWRITE_TAC [] ],
       (* goal 2 (of 2) *)
       Cases_on `u` >| (* 2 sub-goals here *)
       [ (* goal 2.1 (of 2) *)
         PAT_X_ASSUM ``WEAK_EQUIV p q``
-		  (STRIP_ASSUME_TAC o (ONCE_REWRITE_RULE [OBS_PROPERTY_STAR])) \\
+		  (STRIP_ASSUME_TAC o (ONCE_REWRITE_RULE [WEAK_PROPERTY_STAR])) \\
         RES_TAC \\
         IMP_RES_TAC EPS_cases1 >- PROVE_TAC [] \\
         Q.EXISTS_TAC `E1` >> ASM_REWRITE_TAC [] \\
@@ -79,7 +80,7 @@ val DENG_LEMMA = store_thm ((* NEW *)
         take [`p`, `u`] >> ASM_REWRITE_TAC [EPS_REFL, PREFIX],
         (* goal 1.2.2 (of 2) *)
         PAT_X_ASSUM ``WEAK_EQUIV p q``
-		  (STRIP_ASSUME_TAC o (ONCE_REWRITE_RULE [OBS_PROPERTY_STAR])) \\
+		  (STRIP_ASSUME_TAC o (ONCE_REWRITE_RULE [WEAK_PROPERTY_STAR])) \\
         RES_TAC \\
         Q.EXISTS_TAC `E1` >> ASM_REWRITE_TAC [] ] ]);
 
@@ -88,7 +89,7 @@ val HENNESSY_LEMMA_RL = store_thm ((* NEW *)
    "HENNESSY_LEMMA_RL",
   ``!p q. (OBS_CONGR p q \/ OBS_CONGR p (prefix tau q) \/
 			    OBS_CONGR (prefix tau p) q) ==> WEAK_EQUIV p q``,
-    REPEAT STRIP_TAC (* 3 sub-goals here *)
+    rpt STRIP_TAC (* 3 sub-goals here *)
  >| [ (* goal 2.1 (of 3) *)
       IMP_RES_TAC OBS_CONGR_IMP_WEAK_EQUIV,
       (* goal 2.2 (of 3) *)
@@ -106,7 +107,7 @@ val HENNESSY_LEMMA_LR = store_thm ((* NEW *)
    "HENNESSY_LEMMA_LR",
   ``!p q. WEAK_EQUIV p q ==> (OBS_CONGR p q \/ OBS_CONGR p (prefix tau q)
 					    \/ OBS_CONGR (prefix tau p) q)``,
-    REPEAT STRIP_TAC
+    rpt STRIP_TAC
  >> Cases_on `?E. TRANS p tau E /\ WEAK_EQUIV E q` (* 2 sub-goals here *)
  >| [ (* goal 1 (of 2) *)
       DISJ2_TAC >> DISJ1_TAC \\ (* CHOOSE ``p ~~c tau..q`` *)
@@ -114,7 +115,7 @@ val HENNESSY_LEMMA_LR = store_thm ((* NEW *)
       [ (* goal 1.1 (of 2) *)
         Cases_on `u` \\ (* 2 sub-goals here, sharing initial tacticals *)
         PAT_X_ASSUM ``WEAK_EQUIV p q``
-		    (STRIP_ASSUME_TAC o (ONCE_REWRITE_RULE [OBS_PROPERTY_STAR])) \\
+		    (STRIP_ASSUME_TAC o (ONCE_REWRITE_RULE [WEAK_PROPERTY_STAR])) \\
         RES_TAC \\
         Q.EXISTS_TAC `E2` >> ASM_REWRITE_TAC [] >|
         [ (* goal 1.1.1 (of 2) *)
@@ -142,7 +143,7 @@ val HENNESSY_LEMMA_LR = store_thm ((* NEW *)
           (* goal 2.1.2 (of 2) *)
           Cases_on `u` \\ (* 2 sub-goals here, sharing initial tacticals *)
           PAT_X_ASSUM ``WEAK_EQUIV p q``
-		      (STRIP_ASSUME_TAC o (ONCE_REWRITE_RULE [OBS_PROPERTY_STAR])) \\
+		      (STRIP_ASSUME_TAC o (ONCE_REWRITE_RULE [WEAK_PROPERTY_STAR])) \\
           RES_TAC \\
           Q.EXISTS_TAC `E1` >> ASM_REWRITE_TAC [] >|
           [ (* goal 2.1.2.1 (of 2) *)
@@ -161,20 +162,17 @@ val HENNESSY_LEMMA = store_thm ((* NEW *)
    "HENNESSY_LEMMA",
   ``!p q. WEAK_EQUIV p q = (OBS_CONGR p q \/ OBS_CONGR p (prefix tau q)
 					  \/ OBS_CONGR (prefix tau p) q)``,
-    REPEAT GEN_TAC
- >> EQ_TAC (* 2 sub-goals here *)
- >| [ (* goal 1 (of 2), hard part *)
-      REWRITE_TAC [HENNESSY_LEMMA_LR],
-      (* goal 2 (of 2), easy part *)
-      REWRITE_TAC [HENNESSY_LEMMA_RL] ]);
+    rpt GEN_TAC >> EQ_TAC
+ >- REWRITE_TAC [HENNESSY_LEMMA_LR]
+ >> REWRITE_TAC [HENNESSY_LEMMA_RL]);
 
 (* Definition 12: the coarsest congruence that is finer than WEAK_EQUIV is called
                   WEAK_CONGR (weak bisimulation congruence) *)
 val WEAK_CONGR = new_definition ((* NEW *)
    "WEAK_CONGR", ``WEAK_CONGR = CC WEAK_EQUIV``);
 
-val WEAK_CONGR_thm = save_thm (
-   "WEAK_CONGR_thm", REWRITE_RULE [CC_def] WEAK_CONGR);
+val WEAK_CONGR_THM = save_thm (
+   "WEAK_CONGR_THM", REWRITE_RULE [CC_def] WEAK_CONGR);
 
 val WEAK_CONGR_congruence = store_thm ((* NEW *)
    "WEAK_CONGR_congruence", ``congruence WEAK_CONGR``,
@@ -216,7 +214,7 @@ val WEAK_CONGR_IMP_SUM_EQUIV = store_thm ((* NEW *)
 val COARSEST_CONGR_LR = store_thm ((* NEW *)
    "COARSEST_CONGR_LR",
   ``!p q. OBS_CONGR p q ==> !r. WEAK_EQUIV (sum p r) (sum q r)``,
-    REPEAT STRIP_TAC
+    rpt STRIP_TAC
  >> MATCH_MP_TAC OBS_CONGR_IMP_WEAK_EQUIV
  >> RW_TAC std_ss [OBS_CONGR_SUBST_SUM_R]);
 
@@ -229,7 +227,7 @@ val COARSEST_CONGR_RL = store_thm ((* NEW *)
   ``!p q. free_action p /\ free_action q ==>
 	  (!r. WEAK_EQUIV (sum p r) (sum q r)) ==> OBS_CONGR p q``,
     REWRITE_TAC [free_action_def, OBS_CONGR]
- >> REPEAT STRIP_TAC (* 2 sub-goals here *)
+ >> rpt STRIP_TAC (* 2 sub-goals here *)
  >| [ (* goal 1 (of 2) *)
       ASSUME_TAC (Q.SPEC `prefix (label a) nil`
 			 (ASSUME ``!r. WEAK_EQUIV (sum p r) (sum q r)``)) \\
@@ -238,7 +236,7 @@ val COARSEST_CONGR_RL = store_thm ((* NEW *)
       Cases_on `u` >| (* 2 sub-goals here *)
       [ (* goal 1.1 (of 2) *)
         STRIP_ASSUME_TAC
-          (ONCE_REWRITE_RULE [OBS_PROPERTY_STAR]
+          (ONCE_REWRITE_RULE [WEAK_PROPERTY_STAR]
 			     (ASSUME ``WEAK_EQUIV (sum p (prefix (label a) nil))
 						  (sum q (prefix (label a) nil))``)) \\
         RES_TAC \\
@@ -246,7 +244,7 @@ val COARSEST_CONGR_RL = store_thm ((* NEW *)
         [ (* goal 1.1.1 (of 2) *)
           `TRANS E2 (label a) nil` by RW_TAC std_ss [SUM2, PREFIX] \\
           STRIP_ASSUME_TAC
-            (ONCE_REWRITE_RULE [OBS_PROPERTY_STAR] (ASSUME ``WEAK_EQUIV E1 E2``)) \\
+            (ONCE_REWRITE_RULE [WEAK_PROPERTY_STAR] (ASSUME ``WEAK_EQUIV E1 E2``)) \\
           RES_TAC \\
           IMP_RES_TAC TRANS_TAU_AND_WEAK \\
           RES_TAC,				(* initial assumption of `p` is used here *)
@@ -262,7 +260,7 @@ val COARSEST_CONGR_RL = store_thm ((* NEW *)
             RW_TAC std_ss [Action_distinct] ] ],
         (* goal 1.2 (of 2) *)
         STRIP_ASSUME_TAC
-          (ONCE_REWRITE_RULE [OBS_PROPERTY_STAR]
+          (ONCE_REWRITE_RULE [WEAK_PROPERTY_STAR]
 			     (ASSUME ``WEAK_EQUIV (sum p (prefix (label a) nil))
 						  (sum q (prefix (label a) nil))``)) \\
         RES_TAC \\
@@ -298,7 +296,7 @@ val COARSEST_CONGR_RL = store_thm ((* NEW *)
       Cases_on `u` >| (* 2 sub-goals here *)
       [ (* goal 2.1 (of 2) *)
         STRIP_ASSUME_TAC
-          (ONCE_REWRITE_RULE [OBS_PROPERTY_STAR]
+          (ONCE_REWRITE_RULE [WEAK_PROPERTY_STAR]
 			     (ASSUME ``WEAK_EQUIV (sum p (prefix (label a') nil))
 						  (sum q (prefix (label a') nil))``)) \\
         RES_TAC \\
@@ -306,7 +304,7 @@ val COARSEST_CONGR_RL = store_thm ((* NEW *)
         [ (* goal 2.1.1 (of 2) *)
           `TRANS E1 (label a') nil` by RW_TAC std_ss [SUM2, PREFIX] \\
           STRIP_ASSUME_TAC
-            (ONCE_REWRITE_RULE [OBS_PROPERTY_STAR] (ASSUME ``WEAK_EQUIV E1 E2``)) \\
+            (ONCE_REWRITE_RULE [WEAK_PROPERTY_STAR] (ASSUME ``WEAK_EQUIV E1 E2``)) \\
           RES_TAC \\
           IMP_RES_TAC TRANS_TAU_AND_WEAK \\
           RES_TAC,				(* initial assumption of `q` is used here *)
@@ -322,7 +320,7 @@ val COARSEST_CONGR_RL = store_thm ((* NEW *)
             RW_TAC std_ss [Action_distinct] ] ],
         (* goal 2.2 (of 2) *)
         STRIP_ASSUME_TAC
-          (ONCE_REWRITE_RULE [OBS_PROPERTY_STAR]
+          (ONCE_REWRITE_RULE [WEAK_PROPERTY_STAR]
 			     (ASSUME ``WEAK_EQUIV (sum p (prefix (label a') nil))
 						  (sum q (prefix (label a') nil))``)) \\
         RES_TAC \\
@@ -357,7 +355,7 @@ val COARSEST_CONGR_THM = store_thm ((* NEW *)
    "COARSEST_CONGR_THM",
   ``!p q. free_action p /\ free_action q ==>
 	  (OBS_CONGR p q = !r. WEAK_EQUIV (sum p r) (sum q r))``,
-    REPEAT STRIP_TAC
+    rpt STRIP_TAC
  >> EQ_TAC >- REWRITE_TAC [COARSEST_CONGR_LR]
  >> MATCH_MP_TAC COARSEST_CONGR_RL
  >> ASM_REWRITE_TAC []);
@@ -375,16 +373,16 @@ val PROP3_COMMON = store_thm ((* NEW *)
 	       (!p' u. WEAK_TRANS p u p' ==> ~(WEAK_EQUIV p' k)) /\
 	       (!q' u. WEAK_TRANS q u q' ==> ~(WEAK_EQUIV q' k))) ==>
           (!r. WEAK_EQUIV (sum p r) (sum q r)) ==> OBS_CONGR p q``,
-    REPEAT STRIP_TAC
+    rpt STRIP_TAC
  >> PAT_X_ASSUM ``!r. WEAK_EQUIV (sum p r) (sum q r)``
 		(ASSUME_TAC o (Q.SPEC `prefix (label a) k`))
  >> REWRITE_TAC [OBS_CONGR]
- >> REPEAT STRIP_TAC (* 2 sub-goals here *)
+ >> rpt STRIP_TAC (* 2 sub-goals here *)
  >| [ (* goal 1 (of 2) *)
       IMP_RES_TAC SUM1 \\
       POP_ASSUM (ASSUME_TAC o (Q.SPEC `prefix (label a) k`)) \\
       PAT_X_ASSUM ``WEAK_EQUIV (sum p (prefix (label a) k)) (sum q (prefix (label a) k))``
-	(STRIP_ASSUME_TAC o (ONCE_REWRITE_RULE [OBS_PROPERTY_STAR])) \\
+	(STRIP_ASSUME_TAC o (ONCE_REWRITE_RULE [WEAK_PROPERTY_STAR])) \\
       Cases_on `u` >| (* 2 sub-goals here *)
       [ (* goal 1.1 (of 2) *)
         RES_TAC \\
@@ -393,7 +391,7 @@ val PROP3_COMMON = store_thm ((* NEW *)
         [ (* goal 1.1.1 (of 2) *)
           `TRANS E2 (label a) k` by PROVE_TAC [PREFIX, SUM2] \\
           PAT_X_ASSUM ``WEAK_EQUIV E1 E2``
-	    (STRIP_ASSUME_TAC o (ONCE_REWRITE_RULE [OBS_PROPERTY_STAR])) \\
+	    (STRIP_ASSUME_TAC o (ONCE_REWRITE_RULE [WEAK_PROPERTY_STAR])) \\
           RES_TAC \\
           IMP_RES_TAC TRANS_TAU_AND_WEAK \\
           PROVE_TAC [],
@@ -454,7 +452,7 @@ val PROP3_COMMON = store_thm ((* NEW *)
       IMP_RES_TAC SUM1 \\
       POP_ASSUM (ASSUME_TAC o (Q.SPEC `prefix (label a) k`)) \\
       PAT_X_ASSUM ``WEAK_EQUIV (sum p (prefix (label a) k)) (sum h (prefix (label a) k))``
-	(STRIP_ASSUME_TAC o (ONCE_REWRITE_RULE [OBS_PROPERTY_STAR])) \\
+	(STRIP_ASSUME_TAC o (ONCE_REWRITE_RULE [WEAK_PROPERTY_STAR])) \\
       Cases_on `u` >| (* 2 sub-goals here *)
       [ (* goal 2.1 (of 2) *)
         RES_TAC \\
@@ -463,7 +461,7 @@ val PROP3_COMMON = store_thm ((* NEW *)
         [ (* goal 2.1.1 (of 2) *)
           `TRANS E1 (label a) k` by PROVE_TAC [PREFIX, SUM2] \\
           PAT_X_ASSUM ``WEAK_EQUIV E1 E2``
-	    (STRIP_ASSUME_TAC o (ONCE_REWRITE_RULE [OBS_PROPERTY_STAR])) \\
+	    (STRIP_ASSUME_TAC o (ONCE_REWRITE_RULE [WEAK_PROPERTY_STAR])) \\
           RES_TAC \\
           IMP_RES_TAC TRANS_TAU_AND_WEAK \\
           `WEAK_EQUIV E2' k` by PROVE_TAC [WEAK_EQUIV_SYM] \\ (* one extra step *)
@@ -532,7 +530,7 @@ val KLOP_def = Define `
 
 val K0_NO_TRANS = store_thm (
    "K0_NO_TRANS", ``!(a :'b Label) u E. ~(TRANS (KLOP a 0) u E)``,
-    REPEAT GEN_TAC
+    rpt GEN_TAC
  >> REWRITE_TAC [KLOP_def]
  >> REWRITE_TAC [NIL_NO_TRANS]);
 
@@ -544,7 +542,7 @@ val KLOP_PROP0 = store_thm ((* NEW *)
  >- REWRITE_TAC [STABLE, KLOP_def, NIL_NO_TRANS]
  >> POP_ASSUM MP_TAC
  >> REWRITE_TAC [STABLE, KLOP_def]
- >> REPEAT STRIP_TAC
+ >> rpt STRIP_TAC
  >> IMP_RES_TAC TRANS_SUM (* 2 sub-goals here *)
  >- PROVE_TAC []
  >> IMP_RES_TAC TRANS_PREFIX
@@ -559,7 +557,7 @@ val KLOP_PROP1_LR = store_thm ((* NEW *)
  >> Induct_on `n` (* 2 sub-goals here, first one is easy *)
  >- PROVE_TAC [K0_NO_TRANS]
  >> REWRITE_TAC [KLOP_def]
- >> REPEAT STRIP_TAC
+ >> rpt STRIP_TAC
  >> IMP_RES_TAC TRANS_SUM (* 2 sub-goals here *)
  >| [ (* goal 1 (of 2) *)
       RES_TAC \\
@@ -577,7 +575,7 @@ val KLOP_PROP1_RL = store_thm ((* NEW *)
   ``!(a :'b Label) n E. (?m. m < n /\ (E = KLOP a m)) ==> TRANS (KLOP a n) (label a) E``,
     GEN_TAC
  >> Induct_on `n` (* 2 sub-goals here *)
- >> REPEAT STRIP_TAC
+ >> rpt STRIP_TAC
  >- IMP_RES_TAC NOT_LESS_0
  >> REWRITE_TAC [KLOP_def]
  >> IMP_RES_TAC LESS_LEMMA1 (* 2 sub-goals here *)
@@ -592,7 +590,7 @@ val KLOP_PROP1_RL = store_thm ((* NEW *)
 val KLOP_PROP1 = store_thm ((* NEW *)
    "KLOP_PROP1",
   ``!(a :'b Label) n E. TRANS (KLOP a n) (label a) E = (?m. m < n /\ (E = KLOP a m))``,
-    REPEAT GEN_TAC
+    rpt GEN_TAC
  >> EQ_TAC (* 2 sub-goals here *)
  >| [ (* goal 1 (of 2) *)
       REWRITE_TAC [KLOP_PROP1_LR],
@@ -603,7 +601,7 @@ val KLOP_PROP1 = store_thm ((* NEW *)
 val KLOP_PROP1' = store_thm ((* NEW *)
    "KLOP_PROP1'",
   ``!(a :'b Label) n E.	WEAK_TRANS (KLOP a n) (label a) E = (?m. m < n /\ (E = KLOP a m))``,
-    REPEAT GEN_TAC
+    rpt GEN_TAC
  >> EQ_TAC (* 2 sub-goals here *)
  >| [ (* goal 1 (of 2) *)
       DISCH_TAC \\
@@ -630,7 +628,7 @@ val KLOP_PROP2 = store_thm ((* NEW *)
   ``!(a :'b Label) n m. m < n ==> ~(STRONG_EQUIV (KLOP a m) (KLOP a n))``,
     GEN_TAC
  >> completeInduct_on `n`
- >> REPEAT STRIP_TAC
+ >> rpt STRIP_TAC
  >> `TRANS (KLOP a n) (label a) (KLOP a m)` by PROVE_TAC [KLOP_PROP1]
  >> STRIP_ASSUME_TAC
 	(((Q.SPEC `label a`) o (ONCE_REWRITE_RULE [PROPERTY_STAR]))
@@ -646,10 +644,10 @@ val KLOP_PROP2' = store_thm ((* NEW *)
   ``!(a :'b Label) n m. m < n ==> ~(WEAK_EQUIV (KLOP a m) (KLOP a n))``,
     GEN_TAC
  >> completeInduct_on `n`
- >> REPEAT STRIP_TAC
+ >> rpt STRIP_TAC
  >> `TRANS (KLOP a n) (label a) (KLOP a m)` by PROVE_TAC [KLOP_PROP1]
  >> STRIP_ASSUME_TAC
-	(ONCE_REWRITE_RULE [OBS_PROPERTY_STAR]
+	(ONCE_REWRITE_RULE [WEAK_PROPERTY_STAR]
 			   (ASSUME ``WEAK_EQUIV (KLOP (a :'b Label) m) (KLOP a n)``))
  >> RES_TAC
  >> PAT_X_ASSUM ``WEAK TRANS (KLOP (a :'b Label) m) (label a) E1``
@@ -660,7 +658,7 @@ val KLOP_ONE_ONE = store_thm ((* NEW *)
    "KLOP_ONE_ONE", ``!(a :'b Label). ONE_ONE (KLOP a)``,
     REWRITE_TAC [ONE_ONE_DEF]
  >> BETA_TAC
- >> REPEAT STRIP_TAC
+ >> rpt STRIP_TAC
  >> IMP_RES_TAC EQUAL_IMP_STRONG_EQUIV
  >> CCONTR_TAC
  >> `x1 < x2 \/ x2 < x1` by PROVE_TAC [LESS_LESS_CASES] (* 2 sub-goals here *)
@@ -702,15 +700,15 @@ val KLOP_ONE_ONE = store_thm ((* NEW *)
  *)
 
 (* The pure Math part in the proof of KLOP_LEMMA_FINITE *)
-val KLOP_EXISTS_LEMMA = store_thm ((* NEW *)
-   "KLOP_EXISTS_LEMMA",
+val INFINITE_EXISTS_LEMMA = store_thm ((* NEW *)
+   "INFINITE_EXISTS_LEMMA",
   ``!R A B. equivalence (R :'a -> 'a -> bool) ==>
          FINITE (A :'a -> bool) /\ INFINITE (B :'a -> bool) /\
          (!x y. x IN B /\ y IN B /\ x <> y ==> ~(R x y)) ==>
        ?k. k IN B /\ (!n. n IN A ==> ~(R n k))``,
-    REPEAT GEN_TAC
+    rpt GEN_TAC
  >> REWRITE_TAC [equivalence_def]
- >> REPEAT STRIP_TAC
+ >> rpt STRIP_TAC
 
  >> Q.ABBREV_TAC `map = (\x. if (?y. y IN B /\ R x y) then
 				(@y. y IN B /\ R x y) else (CHOICE B))`
@@ -731,7 +729,7 @@ val KLOP_EXISTS_LEMMA = store_thm ((* NEW *)
  >> `FINITE B0` by PROVE_TAC [IMAGE_FINITE]
  >> Know `B0 SUBSET B`
  >- ( REWRITE_TAC [SUBSET_DEF] \\
-      REPEAT STRIP_TAC \\
+      rpt STRIP_TAC \\
       `x IN (IMAGE map A)` by PROVE_TAC [] \\
       POP_ASSUM MP_TAC \\
       REWRITE_TAC [IN_IMAGE] >> PROVE_TAC [] ) >> DISCH_TAC
@@ -740,7 +738,7 @@ val KLOP_EXISTS_LEMMA = store_thm ((* NEW *)
  >> Q.EXISTS_TAC `k`
  >> `!n. n IN A ==> map n IN B0` by PROVE_TAC [IN_IMAGE]
  >> Know `!n. n IN A ==> R n (map n) \/ (~?x. x IN B /\ R n x)`
- >- ( REPEAT STRIP_TAC \\
+ >- ( rpt STRIP_TAC \\
       PAT_X_ASSUM ``!x. map x = P`` (ASSUME_TAC o (Q.SPEC `n`)) \\
       Cases_on `?y. y IN B /\ R n y` >| (* 2 sub-goals here *)
       [ (* goal 1 (of 2) *)
@@ -750,7 +748,7 @@ val KLOP_EXISTS_LEMMA = store_thm ((* NEW *)
         (* goal 2 (of 2) *)
         FULL_SIMP_TAC std_ss [] ] ) >> DISCH_TAC
  >> Know `!n. n IN A ==> ~(R n k)`
- >- ( REPEAT STRIP_TAC \\
+ >- ( rpt STRIP_TAC \\
       `map n IN B0` by PROVE_TAC [IMAGE_IN] \\
       Q.ABBREV_TAC `y = map n` \\
       RES_TAC >| (* 2 sub-goals here *)
@@ -770,7 +768,7 @@ val KLOP_LEMMA_FINITE = store_thm ((* NEW *)
 	  ?k. STABLE k /\
 	      (!p' u. WEAK_TRANS p u p' ==> ~(WEAK_EQUIV p' k)) /\
 	      (!q' u. WEAK_TRANS q u q' ==> ~(WEAK_EQUIV q' k))``,
-    REPEAT STRIP_TAC
+    rpt STRIP_TAC
  (* Part 1: assert that the union of all nodes in g and h is finite *)
  >> PAT_X_ASSUM ``finite_state p``
 	(ASSUME_TAC o (REWRITE_RULE [finite_state_def]))
@@ -799,7 +797,7 @@ val KLOP_LEMMA_FINITE = store_thm ((* NEW *)
 *)
  (* Part 3: assert the distincity of elements in the infinite set *)
  >> Know `!x y. x IN klops /\ y IN klops /\ x <> y ==> ~(WEAK_EQUIV x y)`
- >- ( REPEAT STRIP_TAC \\
+ >- ( rpt STRIP_TAC \\
       `?n. x = KLOP a n` by PROVE_TAC [IN_UNIV, IN_IMAGE] \\
       `?m. y = KLOP a m` by PROVE_TAC [IN_UNIV, IN_IMAGE] \\
       STRIP_ASSUME_TAC (Q.SPECL [`m`, `n`] LESS_LESS_CASES) >| (* 3 sub-goals here *)
@@ -815,7 +813,7 @@ val KLOP_LEMMA_FINITE = store_thm ((* NEW *)
  >> POP_ASSUM (MP_TAC o
 	       (MATCH_MP (ISPECL [``WEAK_EQUIV :('a, 'b) simulation``,
 				  ``nodes :('a, 'b) CCS -> bool``,
-				  ``klops :('a, 'b) CCS -> bool``] KLOP_EXISTS_LEMMA)))
+				  ``klops :('a, 'b) CCS -> bool``] INFINITE_EXISTS_LEMMA)))
  >> RW_TAC std_ss []
 (*
   9.  ∀x y. x ∈ klops ∧ y ∈ klops ∧ x ≠ y ⇒ ¬(x ≈ y)
@@ -832,11 +830,11 @@ val KLOP_LEMMA_FINITE = store_thm ((* NEW *)
  >> `!n. n IN (NODES q) ==> ~(WEAK_EQUIV n k)` by PROVE_TAC [IN_UNION]
  >> CONJ_TAC (* 2 sub-goals here *)
  >| [ (* goal 1 (of 2) *)
-      REPEAT STRIP_TAC \\
+      rpt STRIP_TAC \\
       IMP_RES_TAC WEAK_TRANS_IN_NODES \\
       PROVE_TAC [],
       (* goal 2 (of 2) *)
-      REPEAT STRIP_TAC \\
+      rpt STRIP_TAC \\
       IMP_RES_TAC WEAK_TRANS_IN_NODES \\
       PROVE_TAC [] ]);
 
@@ -845,399 +843,10 @@ val COARSEST_CONGR_FINITE = store_thm ((* NEW *)
    "COARSEST_CONGR_FINITE",
   ``!p q. finite_state p /\ finite_state q ==>
 	  (OBS_CONGR p q = !r. WEAK_EQUIV (sum p r) (sum q r))``,
-    REPEAT STRIP_TAC
+    rpt STRIP_TAC
  >> EQ_TAC >- REWRITE_TAC [COARSEST_CONGR_LR]
  >> MP_TAC (Q.SPECL [`p`, `q`] KLOP_LEMMA_FINITE)
  >> RW_TAC std_ss [PROP3_COMMON]);
-
-(******************************************************************************)
-(*                                                                            *)
-(*           Arbitrary Many Non-bisimilar Processes (Klop processes)          *)
-(*                                                                            *)
-(******************************************************************************)
-
-(* `Klop function` has type ``:'b Label -> 'a ordinal -> ('a, 'b) LTS`` *)
-val Klop_def = Define `
-    Klop (l: 'b Label) (n :'a ordinal) =
-	 ABS_graph ({m | m <= n}, {({p}, label l, {q}) | p <= n /\ q < p})`;
-
-val Klop_0 = store_thm ((* NEW *)
-   "Klop_0",
-  ``!(a :'b Label). Klop a 0 = ABS_graph ({0}, EMPTY)``,
-    GEN_TAC >> REWRITE_TAC [Klop_def]
- >> SIMP_TAC std_ss []
- >> Know `hypergraph (({0}, EMPTY) :('a ordinal, 'b Action) REP_graph)`
- >- ( REWRITE_TAC [hypergraph_def] >> SIMP_TAC std_ss [NOT_IN_EMPTY] )
- >> Know `hypergraph (({m | m <= 0}, {({p}, label a, {q}) | p <= 0 /\ q < p})
-		      :('a ordinal, 'b Action) REP_graph)`
- >- ( REWRITE_TAC [hypergraph_def] >> SIMP_TAC std_ss [NOT_IN_EMPTY] \\
-      GEN_TAC >> RW_TAC std_ss [GSPECIFICATION] \\
-      POP_ASSUM MP_TAC \\
-      Cases_on `x` >> FULL_SIMP_TAC std_ss [] \\
-      Cases_on `e` >> Cases_on `r'` \\
-      FULL_SIMP_TAC std_ss [ends_def, inits_def, ters_def, SUBSET_DEF, UNION_DEF,
-			    GSPECIFICATION, IN_SING] \\
-      RW_TAC std_ss [] >- ASM_REWRITE_TAC [] \\
-      REV_FULL_SIMP_TAC std_ss [ordleq0, ordlt_ZERO] )
- >> rpt STRIP_TAC
- >> FULL_SIMP_TAC std_ss [ABS_graph_one_one] >> KILL_TAC
- >> CONJ_TAC (* 2 sub-goals here *)
- >- ( REWRITE_TAC [EXTENSION, GSPECIFICATION, IN_SING] \\
-      GEN_TAC >> EQ_TAC >| (* 2 sub-goals here *)
-      [ (* goal 1 (of 2) *)
-	BETA_TAC >> rpt STRIP_TAC >> FULL_SIMP_TAC std_ss [ordleq0],
-	(* goal 2 (of 2) *)
-	Rewr >> BETA_TAC >> Q.EXISTS_TAC `0` >> SIMP_TAC std_ss [ordlt_REFL] ] )
- >> REWRITE_TAC [EXTENSION, GSPECIFICATION, NOT_IN_EMPTY]
- >> rpt STRIP_TAC
- >> Cases_on `x'` >> FULL_SIMP_TAC std_ss [ordleq0]
- >> REV_FULL_SIMP_TAC std_ss [ordlt_ZERO]);
-
-val Klop_case1 = store_thm ((* NEW *)
-   "Klop_case1",
-  ``!(a :'b Label) (n :'a ordinal) N (u :'b Action) (E :('a, 'b) CCS).
-     ordSUC n <= N ==>
-       (TRANS (lts (ordSUC n) (Klop a N)) u E =
-	((u = label a) /\ (E = lts n (Klop a N))) \/ TRANS (lts n (Klop a N)) u E)``,
-    rpt GEN_TAC
- >> REWRITE_TAC [Klop_def]
- >> Know `hypergraph (({m | m <= N}, {({p}, label a, {q}) | p <= N /\ q < p})
-		      :('a ordinal, 'b Action) REP_graph)`
-    >- ( REWRITE_TAC [hypergraph_def] \\
-	 GEN_TAC >> RW_TAC std_ss [GSPECIFICATION] \\
-	 POP_ASSUM MP_TAC \\
-	 Cases_on `x` >> FULL_SIMP_TAC std_ss [] \\
-	 Cases_on `e` >> Cases_on `r'` \\
-	 FULL_SIMP_TAC std_ss [ends_def, inits_def, ters_def, SUBSET_DEF, UNION_DEF,
-			       GSPECIFICATION, IN_SING] \\
-	 RW_TAC std_ss [] >- art [] \\
-	 MATCH_MP_TAC ordle_TRANS \\
-	 Q.EXISTS_TAC `q` >> art [] \\
-	 REWRITE_TAC [ordle_lteq] >> DISJ1_TAC >> art [] )
- >> rpt STRIP_TAC
- >> EQ_TAC (* 2 sub-goals here *)
- >| [ (* goal 1 (of 2) *)
-      DISCH_TAC \\
-      POP_ASSUM (STRIP_ASSUME_TAC o (SIMP_RULE std_ss [CCS_distinct', CCS_11]) o
-		 (ONCE_REWRITE_RULE [TRANS_cases])) \\
-      rfs [labeled_directed_edges_def, graph_edges_def, graph_REP_ABS, REP_edges_def] \\
-      rfs [labeled_directed_def, init_def, label_def, ter_def, ters_def, inits_def] \\
-      Q.PAT_X_ASSUM `ordSUC n = p` (ASSUME_TAC o SYM) >> fs [] \\
-      Cases_on `q = n` >> art [] \\
-      MATCH_MP_TAC LTS \\
-      fs [labeled_directed_edges_def, graph_edges_def, graph_REP_ABS, REP_edges_def] \\
-      Q.EXISTS_TAC `({n}, label a, {q})` \\
-      fs [labeled_directed_def, init_def, label_def, ter_def, ters_def, inits_def] \\
-      CONJ_TAC >- ( MATCH_MP_TAC ordle_TRANS \\
-		    Q.EXISTS_TAC `ordSUC n` >> art [] \\
-		    REWRITE_TAC [ordle_lteq] >> DISJ1_TAC >> REWRITE_TAC [ordlt_SUC] ) \\
-      fs [ordlt_SUC_DISCRETE],
-      (* goal 2 (of 2) *)
-      rpt STRIP_TAC >> art [] >| (* 2 sub-goals here *)
-      [ (* goal 2.1 (of 2) *)
-	MATCH_MP_TAC LTS \\
-	fs [labeled_directed_edges_def, graph_edges_def, graph_REP_ABS, REP_edges_def] \\
-	Q.EXISTS_TAC `({ordSUC n}, label a, {n})` \\
-	fs [labeled_directed_def, init_def, label_def, ter_def, ters_def, inits_def],
-	(* goal 2.2 (of 2) *)
-	POP_ASSUM (STRIP_ASSUME_TAC o (SIMP_RULE std_ss [CCS_distinct', CCS_11]) o
-		   (ONCE_REWRITE_RULE [TRANS_cases])) >> art [] \\
-	MATCH_MP_TAC LTS \\
-	POP_ASSUM MP_TAC \\
-	fs [labeled_directed_edges_def, graph_edges_def, graph_REP_ABS, REP_edges_def] \\
-	rpt STRIP_TAC \\
-	Q.EXISTS_TAC `({ordSUC n}, u, {E''})` \\
-	fs [labeled_directed_def, init_def, label_def, ter_def, ters_def, inits_def] \\
-	REWRITE_TAC [ordlt_SUC_DISCRETE] >> art [] ] ]);
-
-val Klop_case2 = store_thm ((* NEW *)
-   "Klop_case2",
-  ``!(a :'b Label) (n :'a ordinal) N (u :'b Action) (E :('a, 'b) CCS).
-     0 < n /\ islimit n /\ n <= N ==>
-	(TRANS (lts n (Klop a N)) u E = ?m. m < n /\ TRANS (lts m (Klop a N)) u E)``,
-    rpt STRIP_TAC
- >> RW_TAC std_ss [Klop_def]
- >> Know `hypergraph (({m | m <= N}, {({p}, label a, {q}) | p <= N /\ q < p})
-		      :('a ordinal, 'b Action) REP_graph)`
- >- ( REWRITE_TAC [hypergraph_def] \\
-      GEN_TAC >> RW_TAC std_ss [GSPECIFICATION] \\
-      POP_ASSUM MP_TAC \\
-      Cases_on `x` >> FULL_SIMP_TAC std_ss [] \\
-      Cases_on `e` >> Cases_on `r'` \\
-      FULL_SIMP_TAC std_ss [ends_def, inits_def, ters_def, SUBSET_DEF, UNION_DEF,
-			    GSPECIFICATION, IN_SING] \\
-      RW_TAC std_ss [] >- art [] \\
-      MATCH_MP_TAC ordle_TRANS \\
-      Q.EXISTS_TAC `q` >> art [] \\
-      REWRITE_TAC [ordle_lteq] >> DISJ1_TAC >> art [] )
- >> DISCH_TAC
- >> EQ_TAC (* 2 sub-goals here *)
- >| [ (* goal 1 (of 2) *)
-      rpt STRIP_TAC \\
-      POP_ASSUM (STRIP_ASSUME_TAC o (SIMP_RULE std_ss [CCS_distinct', CCS_11]) o
-		 (ONCE_REWRITE_RULE [TRANS_cases])) \\
-      rfs [labeled_directed_edges_def, graph_edges_def, graph_REP_ABS, REP_edges_def] \\
-      rfs [labeled_directed_def, init_def, label_def, ter_def, ters_def, inits_def] \\
-      fs [] \\
-      IMP_RES_TAC islimit_SUC_lt \\
-      Q.EXISTS_TAC `ordSUC q` >> art [] \\
-      MATCH_MP_TAC LTS \\
-      fs [labeled_directed_edges_def, graph_edges_def, graph_REP_ABS, REP_edges_def] \\
-      Q.EXISTS_TAC `({ordSUC q}, label a, {q})` \\
-      fs [labeled_directed_def, init_def, label_def, ter_def, ters_def, inits_def] \\
-      IMP_RES_TAC ordlte_TRANS \\  
-      REWRITE_TAC [ordle_lteq] >> art [],
-      (* goal 2 (of 2) *)
-      rpt STRIP_TAC \\
-      POP_ASSUM (STRIP_ASSUME_TAC o (SIMP_RULE std_ss [CCS_distinct', CCS_11]) o
-		 (ONCE_REWRITE_RULE [TRANS_cases])) \\
-      rfs [labeled_directed_edges_def, graph_edges_def, graph_REP_ABS, REP_edges_def] \\
-      rfs [labeled_directed_def, init_def, label_def, ter_def, ters_def, inits_def] \\
-      MATCH_MP_TAC LTS \\
-      fs [labeled_directed_edges_def, graph_edges_def, graph_REP_ABS, REP_edges_def] \\
-      Q.EXISTS_TAC `({n}, label a, {q})` \\
-      fs [labeled_directed_def, init_def, label_def, ter_def, ters_def, inits_def] \\
-      IMP_RES_TAC ordlt_TRANS ]);
-
-val Klop_cases = save_thm ((* NEW *)
-   "Klop_cases", LIST_CONJ [Klop_case1, Klop_case2]);
-
-val Klop_rule0 = store_thm ((* NEW *)
-   "Klop_rule0",
-  ``!(a :'b Label) u E (N :'a ordinal). ~(TRANS (lts 0 (Klop a N)) u E)``,
-    RW_TAC std_ss [Klop_def]
- >> Know `hypergraph (({m | m <= N}, {({p}, label a, {q}) | p <= N /\ q < p})
-		      :('a ordinal, 'b Action) REP_graph)`
- >- ( REWRITE_TAC [hypergraph_def] \\
-      GEN_TAC >> RW_TAC std_ss [GSPECIFICATION] \\
-      POP_ASSUM MP_TAC \\
-      Cases_on `x` >> FULL_SIMP_TAC std_ss [] \\
-      Cases_on `e` >> Cases_on `r'` \\
-      FULL_SIMP_TAC std_ss [ends_def, inits_def, ters_def, SUBSET_DEF, UNION_DEF,
-			    GSPECIFICATION, IN_SING] \\
-      RW_TAC std_ss [] >- art [] \\
-      MATCH_MP_TAC ordle_TRANS \\
-      Q.EXISTS_TAC `q` >> art [] \\
-      REWRITE_TAC [ordle_lteq] >> DISJ1_TAC >> art [] )
- >> DISCH_TAC
- >> CCONTR_TAC >> fs []
- >> POP_ASSUM (STRIP_ASSUME_TAC o (SIMP_RULE std_ss [CCS_distinct', CCS_11]) o
-	       (ONCE_REWRITE_RULE [TRANS_cases]))
- >> rfs [labeled_directed_edges_def, graph_edges_def, graph_REP_ABS, REP_edges_def]
- >> rfs [labeled_directed_def, init_def, label_def, ter_def, ters_def, inits_def]
- >> PROVE_TAC [ordlt_ZERO]);
-
-(* Transition rules for Klop processes *)
-val Klop_rule1 = store_thm ((* NEW *)
-   "Klop_rule1",
-  ``!(a :'b Label) (n :'a ordinal) N. (ordSUC n) <= N ==> 
-	TRANS (lts (ordSUC n) (Klop a N)) (label a) (lts n (Klop a N))``,
-    rpt STRIP_TAC
- >> IMP_RES_TAC Klop_case1 >> art []);
-
-val Klop_rule2 = store_thm ((* NEW *)
-   "Klop_rule2",
-  ``!(a :'b Label) (n :'a ordinal) m u (E :('a, 'b) CCS) N.
-	0 < n /\ islimit n /\ n <= N /\ m < n /\ TRANS (lts m (Klop a N)) u E ==>
-		TRANS (lts n (Klop a N)) u E``,
-    rpt STRIP_TAC
- >> IMP_RES_TAC Klop_case2);
-
-val Klop_rules = save_thm ((* NEW *)
-   "Klop_rules", LIST_CONJ [Klop_rule0, Klop_rule1, Klop_rule2]);
-
-val Klop_PROP0 = store_thm ((* NEW *)
-   "Klop_PROP0", ``!(a :'b Label) (n :'a ordinal) N. n <= N ==> STABLE (lts n (Klop a N))``,
-    GEN_TAC
- >> HO_MATCH_MP_TAC simple_ord_induction
- >> rpt STRIP_TAC (* 3 sub-goals here *)
- >| [ (* goal 1 (of 2) *)
-      REWRITE_TAC [STABLE] \\
-      RW_TAC std_ss [Klop_rule0],
-      (* goal 2 (of 3) *)
-      fs [STABLE] >> rpt STRIP_TAC \\
-      `n <= N` by PROVE_TAC [ordlt_SUC, ordle_TRANS, ordle_lteq] \\
-      RES_TAC \\
-      PAT_X_ASSUM ``TRANS (lts (ordSUC n) (Klop a N)) u E'``
-	(STRIP_ASSUME_TAC o (ONCE_REWRITE_RULE [MATCH_MP Klop_case1 (ASSUME ``ordSUC n <= N``)]))
-      >- fs [Action_distinct] >> rfs [],
-      (* goal 3 (of 3) *)
-      fs [STABLE] >> rpt STRIP_TAC \\
-      `?m. m < n /\ TRANS (lts m (Klop a N)) tau E'`
-	  by PROVE_TAC [Q.SPECL [`a`, `n`, `N`, `tau`, `E'`] Klop_case2] \\
-      Q.PAT_X_ASSUM `!n'. n' < n ==> X`
-	  (ASSUME_TAC o (fn thm => MATCH_MP thm (ASSUME ``(m :'a ordinal) < n``))) \\
-      `m <= N` by PROVE_TAC [ordle_lteq, ordle_TRANS] \\
-      RES_TAC ]);
-
-(* Any transition of Klop processes is still a Klop process. Together with Prop 0,
-   this also implies that Klop processes are tau-free. *)
-val Klop_PROP1_LR = store_thm ((* NEW *)
-   "Klop_PROP1_LR",
-  ``!(a :'b Label) (n :'a ordinal) (E :('a, 'b) CCS) N. n <= N ==>
-	TRANS (lts n (Klop a N)) (label a) E ==> ?m. m < n /\ (E = lts m (Klop a N))``,
-    GEN_TAC
- >> HO_MATCH_MP_TAC simple_ord_induction
- >> rpt STRIP_TAC (* 3 sub-goals here *)
- >| [ (* goal 1 (of 3) *)
-      PROVE_TAC [Klop_rule0],
-      (* goal 2 (of 3) *)
-      Q.PAT_X_ASSUM `TRANS (lts (ordSUC n) (Klop a N)) (label a) E`
-	(STRIP_ASSUME_TAC o (ONCE_REWRITE_RULE [MATCH_MP Klop_case1 (ASSUME ``ordSUC n <= N``)]))
-      >- ( Q.EXISTS_TAC `n` >> art [ordlt_SUC] ) \\
-      `n <= N` by PROVE_TAC [ordlt_SUC, ordle_TRANS, ordle_lteq] \\
-      RES_TAC \\
-      Q.EXISTS_TAC `m` >> art [] \\
-      MATCH_MP_TAC ordlt_TRANS \\ 
-      `n < ordSUC n` by PROVE_TAC [ordlt_SUC] \\
-      Q.EXISTS_TAC `n` >> art [],
-      (* goal 3 (of 3) *)
-      MP_TAC (Q.SPECL [`a`, `n`, `N`, `label a`, `E`] Klop_case2) \\
-      RW_TAC std_ss [] \\
-      RES_TAC \\
-      POP_ASSUM K_TAC \\
-      `m <= N` by PROVE_TAC [ordle_TRANS, ordle_lteq] \\
-      Q.PAT_X_ASSUM `!n'. n' < n ==> X`
-	(STRIP_ASSUME_TAC o (fn thm => MATCH_MP thm (ASSUME ``(m :'a ordinal) < n``))) \\
-      POP_ASSUM
-	(STRIP_ASSUME_TAC o (fn thm => MATCH_MP thm (ASSUME ``(m :'a ordinal) <= N``))) \\
-      RES_TAC \\
-      NTAC 2 (POP_ASSUM K_TAC) \\
-      `m' < n` by PROVE_TAC [ordlt_TRANS] \\
-      Q.EXISTS_TAC `m'` >> art [] ]);
-
-val Klop_PROP1_RL = store_thm ((* NEW *)
-   "Klop_PROP1_RL",
-  ``!(a :'b Label) (n :'a ordinal) (E :('a, 'b) CCS) N. n <= N ==>
-	(?m. m < n /\ (E = lts m (Klop a N))) ==> TRANS (lts n (Klop a N)) (label a) E``,
-    GEN_TAC
- >> HO_MATCH_MP_TAC simple_ord_induction
- >> rpt STRIP_TAC (* 3 sub-goals here *)
- >| [ (* goal 1 (of 3) *)
-      PROVE_TAC [ordlt_ZERO],
-      (* goal 2 (of 3) *)
-      `n <= N` by PROVE_TAC [ordlt_SUC, ordle_TRANS, ordle_lteq] \\
-      REWRITE_TAC [MATCH_MP Klop_case1 (ASSUME ``ordSUC n <= N``)] \\
-      PAT_X_ASSUM ``m < ordSUC n``
-	(STRIP_ASSUME_TAC o (REWRITE_RULE [ordlt_SUC_DISCRETE])) >| (* 2 sub-goals here *)
-      [ (* goal 2.1 (of 2) *)
-        DISJ2_TAC >> RES_TAC,
-        (* goal 2.2 (of 2) *)
-        DISJ1_TAC >> art [] ],
-      (* goal 3 (of 3) *)
-      `ordSUC m < n` by PROVE_TAC [islimit_SUC_lt] \\
-      ASSUME_TAC (Q.SPECL [`a`, `m`, `N`] Klop_rule1) \\
-      `ordSUC m <= N` by PROVE_TAC [ordlt_TRANS, ordle_lteq] \\
-      PROVE_TAC [Klop_rule2] ]);
-
-(* Klop processes are closed under transition *)
-val Klop_PROP1 = store_thm ((* NEW *)
-   "Klop_PROP1",
-  ``!(a :'b Label) (n :'a ordinal) (E :('a, 'b) CCS) N. n <= N ==>
-     (TRANS (lts n (Klop a N)) (label a) E = (?m. m < n /\ (E = lts m (Klop a N))))``,
-    rpt STRIP_TAC
- >> EQ_TAC (* 2 sub-goals here *)
- >| [ (* goal 1 (of 2) *)
-      PROVE_TAC [Klop_PROP1_LR],
-      (* goal 2 (of 2) *)
-      PROVE_TAC [Klop_PROP1_RL] ]);
-
-(* Klop processes are closed under weak transition *)
-val Klop_PROP1' = store_thm ((* NEW *)
-   "Klop_PROP1'",
-  ``!(a :'b Label) (n :'a ordinal) (E :('a, 'b) CCS) N. n <= N ==>
-	(WEAK_TRANS (lts n (Klop a N)) (label a) E = (?m. m < n /\ (E = lts m (Klop a N))))``,
-    rpt STRIP_TAC
- >> EQ_TAC (* 2 sub-goals here *)
- >| [ (* goal 1 (of 2) *)
-      DISCH_TAC \\
-      IMP_RES_TAC WEAK_TRANS_cases1 >| (* 2 sub-goals here *)
-      [ (* goal 1.1 (of 2) *)
-        ASSUME_TAC (MATCH_MP (Q.SPECL [`a`, `n`, `N`] Klop_PROP0)
-			     (ASSUME ``(n :'a ordinal) <= N``)) \\
-        IMP_RES_TAC STABLE_NO_TRANS_TAU,
-        (* goal 1.2 (of 2) *)
-        IMP_RES_TAC (MATCH_MP Klop_PROP1_LR (ASSUME ``(n :'a ordinal) <= N``)) \\
-        IMP_RES_TAC EPS_cases1 >| (* 2 sub-goals here *)
-        [ (* goal 1.2.1 (of 2) *)
-          Q.EXISTS_TAC `m` >> PROVE_TAC [],
-          (* goal 1.2.2 (of 2) *)
-          `m <= N` by PROVE_TAC [ordle_TRANS, ordle_lteq] \\
-          ASSUME_TAC (MATCH_MP (Q.SPECL [`a`, `m`, `N`] Klop_PROP0)
-			       (ASSUME ``(m :'a ordinal) <= N``)) \\
-          PROVE_TAC [STABLE_NO_TRANS_TAU] ] ],
-      (* goal 2 (of 2) *)
-      STRIP_TAC \\
-      MATCH_MP_TAC TRANS_IMP_WEAK_TRANS \\
-      RW_TAC std_ss [MATCH_MP (Q.SPECL [`a`, `n`, `E`, `N`] Klop_PROP1_RL)
-			      (ASSUME ``(n :'a ordinal) <= N``)] ]);
-
-(* Klop processes are strongly distinct with each other *)
-val Klop_PROP2 = store_thm ((* NEW *)
-   "Klop_PROP2",
-  ``!(a :'b Label) (n :'a ordinal) m N. m < n /\ n <= N ==>
-	~(STRONG_EQUIV (lts m (Klop a N)) (lts n (Klop a N)))``,
-    GEN_TAC
- >> HO_MATCH_MP_TAC ord_induction
- >> rpt STRIP_TAC
- >> `TRANS (lts n (Klop a N)) (label a) (lts m (Klop a N))` by PROVE_TAC [Klop_PROP1]
- >> PAT_X_ASSUM ``STRONG_EQUIV (lts m (Klop a N)) (lts n (Klop a N))``
-	(STRIP_ASSUME_TAC o (ONCE_REWRITE_RULE [PROPERTY_STAR]))
- >> RES_TAC
- >> `m <= N` by PROVE_TAC [ordle_TRANS, ordle_lteq]
- >> PAT_X_ASSUM ``TRANS (lts m (Klop a N)) (label a) E1``
-	(STRIP_ASSUME_TAC o (REWRITE_RULE [MATCH_MP Klop_PROP1
-						    (ASSUME ``(m :'a ordinal) <= N``)]))
- >> PROVE_TAC []);
-
-(* Klop processes are weakly distinct with each other *)
-val Klop_PROP2' = store_thm ((* NEW *)
-   "Klop_PROP2'",
-  ``!(a :'b Label) (n :'a ordinal) m N. m < n /\ n <= N ==>
-	~(WEAK_EQUIV (lts m (Klop a N)) (lts n (Klop a N)))``,
-    GEN_TAC
- >> HO_MATCH_MP_TAC ord_induction
- >> rpt STRIP_TAC
- >> `TRANS (lts n (Klop a N)) (label a) (lts m (Klop a N))` by PROVE_TAC [Klop_PROP1]
- >> PAT_X_ASSUM ``WEAK_EQUIV (lts m (Klop a N)) (lts n (Klop a N))``
-	(STRIP_ASSUME_TAC o (ONCE_REWRITE_RULE [OBS_PROPERTY_STAR]))
- >> RES_TAC
- >> `m <= N` by PROVE_TAC [ordle_TRANS, ordle_lteq]
- >> PAT_X_ASSUM ``WEAK_TRANS (lts m (Klop a N)) (label a) E1``
-	(STRIP_ASSUME_TAC o (REWRITE_RULE [MATCH_MP Klop_PROP1'
-						    (ASSUME ``(m :'a ordinal) <= N``)]))
- >> PROVE_TAC []);
-
-(* Not used in the project, but this is a beatiful result *)
-val ONE_ONE_IMP_NOTIN = store_thm ((* NEW *)
-   "ONE_ONE_IMP_NOTIN",
-  ``!(A :'a set) (f :'a ordinal -> 'a). ONE_ONE f ==> ?n. f n NOTIN A``,
-    REPEAT GEN_TAC
- >> MP_TAC univ_ord_greater_cardinal
- >> RW_TAC std_ss [ONE_ONE_DEF, cardleq_def, INJ_DEF, IN_UNIV]
- >> CCONTR_TAC
- >> FIRST_X_ASSUM
-	(Q.SPEC_THEN `\n. if n < omega then INL (@m. &m = n) else INR (f n)` MP_TAC)
- >> BETA_TAC
- >> REPEAT STRIP_TAC
- >> Cases_on `x < omega` (* 2 sub-goals here *)
- >| [ (* goal 1 (of 2) *)
-      FULL_SIMP_TAC std_ss [] \\
-      Q.PAT_X_ASSUM `(@m. &m = x) = P` MP_TAC \\
-      REWRITE_TAC [] \\
-      NTAC 2 SELECT_ELIM_TAC \\
-      REPEAT STRIP_TAC >| (* 3 sub-goals here *)
-      [ (* goal 1.1 (of 3) *)
-        Q.PAT_X_ASSUM `y < omega` (ASSUME_TAC o (REWRITE_RULE [lt_omega])) \\
-        PROVE_TAC [],
-        (* goal 1.2 (of 3) *)
-        Q.PAT_X_ASSUM `x < omega` (ASSUME_TAC o (REWRITE_RULE [lt_omega])) \\
-        PROVE_TAC [],
-        (* goal 1.3 (of 3) *)
-        FULL_SIMP_TAC std_ss [] ],
-      (* goal 2 (of 2) *)
-      FULL_SIMP_TAC std_ss [EXTENSION, GSPECIFICATION] \\
-      PROVE_TAC [] ]);
 
 (** Bibliography:
 
